Moved Automation to AutoDB; progress on finalization tatics.

examples/QueryStructure/BookstorewDelegationSemiAutomatic.v
@@ -105,10 +105,6 @@ Definition OrderSchema := QSGetNRelSchemaHeading BookStoreSchema Orders.
 
 (* Now we define an index structure (delegate) for each table. *)
 
-Require Import
-        ADTSynthesis.QueryStructure.Implementation.DataStructures.BagADT.IndexSearchTerms
-        ADTSynthesis.QueryStructure.Implementation.Operations.BagADT.Refinements
-        ADTSynthesis.QueryStructure.Implementation.DataStructures.BagADT.QueryStructureImplementation.
 
 (* Definition OrderSearchTerm := BuildIndexSearchTerm [ OrderSchema/sISBN  ].
 
@@ -146,569 +142,6 @@ Proof.
 Qed. *)
 
 Opaque CallBagMethod.
-
-Arguments BuildIndexSearchTerm : simpl never.
-Arguments MatchIndexSearchTerm : simpl never.
-Opaque Initialize_IndexedQueryStructure.
-
-Ltac fields storage :=
-  match eval cbv delta [storage] in storage with
-  | let src := ?X in _ => X
-  end.
-
-  Ltac prove_extensional_eq :=
-  clear;
-  unfold ExtensionalEq;
-  destruct_ifs; first [ solve [intuition] | solve [exfalso; intuition] | idtac ].
-
-
-Ltac findMatchingTerm fds s k :=
-  match fds with
-    | (?fd, ?X) =>
-      let H := fresh in assert (H : bindex s = fd) by reflexivity; clear H;
-        k X
-    | (?fds1, ?fds2) => findMatchingTerm fds1 s k || findMatchingTerm fds2 s k
-  end.
-
-Ltac createTerm f fds tail fs k :=
-  match fs with
-  | nil =>
-    k tail
-  | ?s :: ?fs' =>
-    createTerm f fds tail fs' ltac:(fun rest =>
-      findMatchingTerm fds s ltac:(fun X =>
-        k (Some X, rest))
-      || k (@None (f s), rest))
-  end.
-
-(* Get the heading of SC, then *)
-Ltac makeTerm fs SC fds tail k :=
-  match eval hnf in SC with
-  | Build_Heading ?f =>
-    createTerm f fds tail fs k
-  end.
-
-(* Given a storage schema [SC], a filter [F], and a
-   tactic [k] which processes filters, convert [F] into
-   a search term (a list of boolean functions over the tuples in
-   [SC]. *)
-Ltac findGoodTerm SC F k :=
-  match F with
-    | fun a => ?[@?f a] =>
-      match type of f with
-        | forall a, {?X = _!?fd} + {_} => k (fd, X) (fun _ : @Tuple SC => true)
-        | forall a, {_!?fd = ?X} + {_} => k (fd, X) (fun _ : @Tuple SC => true)
-        | forall a, {?X = _``?fd} + {_} => k (fd, X) (fun _ : @Tuple SC => true)
-        | forall a, {_``?fd = ?X} + {_} => k (fd, X) (fun _ : @Tuple SC => true)
-      end
-    | fun a => (@?f a) && (@?g a) =>
-      findGoodTerm SC f ltac:(fun fds1 tail1 =>
-                                findGoodTerm SC g ltac:(fun fds2 tail2 =>
-                                                          k (fds1, fds2) (fun tup : @Tuple SC => (tail1 tup) && (tail2 tup))))
-    | _ => k tt F
-  end.
-
-Ltac find_simple_search_term qs_schema idx filter_dec search_term :=
-  match type of search_term with
-    | BuildIndexSearchTerm ?attr =>
-     let SC := constr:(QSGetNRelSchemaHeading qs_schema idx) in
-              findGoodTerm SC filter_dec
-                           ltac:(fun fds tail =>
-                                   let tail := eval simpl in tail in
-                                       makeTerm attr SC fds tail
-                                                ltac:(fun tm => pose tm; try unify tm search_term;
-                                                      unfold ExtensionalEq, MatchIndexSearchTerm;
-                                                      simpl; intro; try prove_extensional_eq))
-  end.
-
-Ltac implement_QSDeletedTuples find_search_term :=
-match goal with
-    [ H : @DelegateToBag_AbsR ?qs_schema ?indices ?r_o ?r_n
-      |- context[Pick (QSDeletedTuples ?r_o ?idx ?DeletedTuples)] ] =>
-    let filter_dec := eval simpl in (@DecideableEnsembles.dec _ DeletedTuples _) in
-    let idx_search_update_term := eval simpl in (ith_Bounded relName indices idx) in
-    let search_term_type := eval simpl in (BagSearchTermType idx_search_update_term) in
-    let search_term_matcher := eval simpl in (BagMatchSearchTerm idx_search_update_term) in
-        makeEvar search_term_type
-                 ltac: (fun search_term =>
-          let eqv := fresh in
-          assert (ExtensionalEq filter_dec (search_term_matcher search_term)) as eqv;
-            [ find_search_term qs_schema idx filter_dec search_term
-            | let H' := fresh in
-              pose (@refine_BagADT_QSDelete_fst _ _ r_o r_n H idx DeletedTuples _ search_term) as H';
-                setoid_rewrite (H' eqv); clear H' eqv])
-end.
-
-Ltac implement_EnsembleDelete_AbsR find_search_term :=
-  match goal with
-      [ H : @DelegateToBag_AbsR ?qs_schema ?indices ?r_o ?r_n
-        |- context[{r_n' | DelegateToBag_AbsR
-                             (UpdateUnConstrRelation ?r_o ?idx
-                                                     (EnsembleDelete (GetUnConstrRelation ?r_o ?idx)
-                                                                     ?DeletedTuples)) r_n'}]] =>
-      let filter_dec := eval simpl in (@DecideableEnsembles.dec _ DeletedTuples _) in
-      let idx_search_update_term := eval simpl in (ith_Bounded relName indices idx) in
-      let search_term_type := eval simpl in (BagSearchTermType idx_search_update_term) in
-      let search_term_matcher := eval simpl in (BagMatchSearchTerm idx_search_update_term) in
-          makeEvar search_term_type
-                   ltac:(fun search_term =>
-                           let eqv := fresh in
-                           assert (ExtensionalEq filter_dec (search_term_matcher search_term)) as eqv;
-                         [ find_search_term qs_schema idx filter_dec search_term
-                         | let H' := fresh in
-                           pose (@refine_BagADT_QSDelete_snd _ _ r_o r_n H idx DeletedTuples _ search_term) as H';
-                             setoid_rewrite (H' eqv); clear H' eqv] )
-  end.
-
-Ltac implement_Enumerate_filter find_search_term :=
-  match goal with
-      [ H : @DelegateToBag_AbsR ?qs_schema ?indices ?r_o ?r_n
-        |- context[For (l <- CallBagMethod ?idx {| bindex := "Enumerate"|} ?r_n0 ();
-                        (List_Query_In (filter (@DecideableEnsembles.dec _ ?DeletedTuples _) (snd l))
-                                            ?resultComp))]] =>
-      let filter_dec := eval simpl in (@DecideableEnsembles.dec _ DeletedTuples _) in
-      let idx_search_update_term := eval simpl in (ith_Bounded relName indices idx) in
-      let search_term_type := eval simpl in (BagSearchTermType idx_search_update_term) in
-      let search_term_matcher := eval simpl in (BagMatchSearchTerm idx_search_update_term) in
-          makeEvar search_term_type
-                   ltac:(fun search_term =>
-                           let eqv := fresh in
-                           assert (ExtensionalEq filter_dec (search_term_matcher search_term)) as eqv;
-                         [ find_search_term qs_schema idx filter_dec search_term
-                         | let H' := fresh in
-                           pose (@refine_Query_For_In_Find _ _ string _ _ H idx filter_dec
-                                                           search_term resultComp) as H';
-                         setoid_rewrite (H' eqv); clear H'])
-  end.
-
-Ltac implement_Pick_DelegateToBag_AbsR_observer :=
-  match goal with
-      [H : @DelegateToBag_AbsR ?qs_schema ?indices ?r_o ?r_n
-       |- context[{r_n' : IndexedQueryStructure ?qs_schema ?indices | DelegateToBag_AbsR ?r_o r_n'}] ]
-      => setoid_rewrite (refine_pick_val (@DelegateToBag_AbsR qs_schema indices r_o) H)
-  end.
-
-  Add Parametric Morphism
-      (A : Type)
-      (f : A -> Type)
-      (As : list A)
-      (a : A)
-      (l' : list (ilist f As))
-      : (@Join_Lists A f As a l')
-      with signature
-      (pointwise_relation _ refine) ==> refine
-        as refine_Join_Lists.
-  Proof.
-    unfold pointwise_relation; simpl; intros.
-    induction l'; unfold Join_Lists; simpl.
-    - reflexivity.
-    - rewrite H; setoid_rewrite IHl'; reflexivity.
-  Qed.
-
-Lemma refine_Join_Enumerate_Swap
-      qs_schema BagIndexKeys
-        (ResultT : Type) :
-    forall r_o (r_n : IndexedQueryStructure qs_schema BagIndexKeys),
-      DelegateToBag_AbsR r_o r_n ->
-      forall (idx idx' : BoundedString)
-             (resultComp : _ -> Comp (list ResultT)),
-        refine (l <- CallBagMethod idx {|bindex := "Enumerate" |} r_n ();
-                l' <- (Join_Lists (Build_single_Tuple_list (snd l))
-                                  (fun _ => l <- (CallBagMethod idx' {|bindex := "Enumerate" |} r_n ());
-                                   ret (snd l)));
-                List_Query_In l' resultComp)
-               (l <- CallBagMethod idx' {|bindex := "Enumerate" |} r_n ();
-                l' <- (Join_Lists (Build_single_Tuple_list (snd l))
-                                  (fun _ => l <- (CallBagMethod idx {|bindex := "Enumerate" |} r_n ());
-                                   ret (snd l)));
-                List_Query_In l' (fun tup_pair => (resultComp (icons _ (ilist_hd (ilist_tl tup_pair)) (icons _ (ilist_hd tup_pair) (inil _)))))).
-  Proof.
-  Admitted.
-
-(* implement_In' implements [UnConstrQuery_In] in a variety of contexts. *)
-Ltac implement_In' :=
-  match goal with
-    (* Implement a List_Query_In of a list [l] applied to a UnConstrQuery_In [idx]
-        by enumerating [idx] with a method call and joining the result with [l] *)
-    | [H : @DelegateToBag_AbsR ?qs_schema ?indexes ?r_o ?r_n
-       |- context[fun b' : ?ElementT => List_Query_In (@?l b') (fun b => UnConstrQuery_In (ResultT := ?resultT) ?r_o ?idx (@?f b' b) )] ] =>
-      let H' := eval simpl in
-      (fun (b' : ElementT) => refine_Join_Query_In_Enumerate' H idx (f b') (l b')) in
-          setoid_rewrite H'
-
-    (* Implement a 'naked' UnConstrQuery_In as a call to enumerate *)
-    | [H : @DelegateToBag_AbsR ?qs_schema ?indexes ?r_o ?r_n
-       |- context[UnConstrQuery_In (ResultT := ?resultT) ?r_o ?idx ?f] ] =>
-      let H' := eval simpl in (refine_Query_In_Enumerate H (idx := idx) f) in
-          setoid_rewrite H'
-
-    (* Implement a UnConstrQuery_In under a single binder as a call to enumerate *)
-    | [H : @DelegateToBag_AbsR ?qs_schema ?indexes ?r_o ?r_n
-       |- context[fun b => UnConstrQuery_In (ResultT := ?resultT) ?r_o ?idx (@?f b) ] ] =>
-      let H' := eval simpl in
-      (fun b => @refine_Query_In_Enumerate qs_schema indexes _ r_o r_n H idx (f b)) in
-          setoid_rewrite H'
-  end.
-
-Ltac implement_In :=
-  (* First simplify any large terms [i.e. Rep, BagSpec, snd, and MethodDomCod
-     that might slow down setoid rewriting *)
-  simpl in *;
-  (* The repeatedly implement [In]s *)
-  repeat implement_In'.
-
-
-  Fixpoint Join_ListsT (Ts : list Type) : Type
-    :=
-      match Ts with
-        | [] => unit
-        | [A] => A
-        | A :: Cs => prod A (Join_ListsT Cs)
-      end.
-
-  Lemma ExtensionalEq_andb {A} :
-    forall (f g f' g' : A -> bool),
-      ExtensionalEq f f'
-      -> ExtensionalEq g g'
-      -> ExtensionalEq (fun a => f a && g a) (fun a => f' a && g' a).
-  Proof.
-    unfold ExtensionalEq; intros; congruence.
-  Qed.
-
-  Lemma ExtensionalEq_andb_true {A} :
-    forall (f f' : A -> bool),
-      ExtensionalEq f f'
-      -> ExtensionalEq f (fun a => f' a && (fun _ => true) a).
-  Proof.
-    unfold ExtensionalEq; intros.
-    rewrite andb_true_r; apply H.
-  Qed.
-
-  Ltac split_filters k :=
-    match goal with
-      | |- ExtensionalEq (fun a => (@?f a) && (@?g a)) ?b =>
-        let fT := type of f in
-        let gT := type of g in
-        makeEvar
-          fT
-          ltac:(fun f' =>
-                  makeEvar gT ltac:(fun g' =>
-                                      apply (@ExtensionalEq_andb _ f g f' g');
-                                    [ first [split_filters | k ] | first [split_filters | k]] ))
-      | |- ExtensionalEq (fun a => (@?f a)) ?b =>
-        let fT := type of f in
-        makeEvar
-          fT
-          ltac:(fun f' => k)
-    end.
-
-  (* Convert List_Query_In Where Clauses into a filter using search terms. *)
-  Ltac convert_Where_to_search_term :=
-    (* First replace Where clauses with test functions. *)
-    simpl; repeat (setoid_rewrite refine_List_Query_In_Where;
-                   instantiate (1 := _)); simpl;
-    (* Combine different filters into a single function. *)
-    repeat setoid_rewrite <- filter_and;
-    (* Now break the functions up again and find search term replacements for each. *)
-    match goal with
-        |- context [List_Query_In (filter ?f _) _] =>
-        let T := type of f in
-        makeEvar T
-                 ltac:(fun g =>
-                         let eqv := fresh in
-                         assert (ExtensionalEq f g) as eqv;
-                       [ apply ExtensionalEq_andb_true; split_filters idtac
-                       | setoid_rewrite (filter_by_equiv f g eqv)])
-    end.
-
-  Ltac equate X Y := let H := fresh in assert (H : X = Y) by reflexivity; clear H.
-
-    Definition unit_Heading :=
-      {| Attributes := unit;
-         Domain := fun _ => unit |}.
-
-    Definition unit_Tuple : @Tuple unit_Heading := id.
-
-    Ltac get_ithDefault f n k :=
-      match type of f with
-        | ilist (@Tuple) ?A -> ?C =>
-          let G := fresh "G" in
-          let p := fresh "p" in
-          let H := fresh "H" in
-          let proj := fresh "proj" in
-          let proj := eval simpl in
-          (fun b : ilist (@Tuple) A => ith_default unit_Heading unit_Tuple b n) in
-          evar (G : @Tuple (nth_default unit_Heading A n) -> C);
-             assert (H : forall p,
-                          f p = G (proj p)) by
-              (subst G; intro p;
-               let p' := eval simpl in (proj p) in
-                   pattern p';
-               match goal with
-                 | [ |- (fun t => @?f t = @?g t) _ ] => equate g f; reflexivity
-               end); clear H;
-        let G' := eval unfold G in G in clear G; k G'
-      end.
-
-    Ltac get_ithDefault_pair f m n k :=
-      match type of f with
-        | ilist (@Tuple) ?A -> ?C =>
-          let G := fresh "G" in
-          let p := fresh "p" in
-          let H := fresh "H" in
-          let proj1 := fresh "proj" in
-          let proj2 := fresh "proj" in
-          let proj1 := eval simpl in
-          (fun b : ilist (@Tuple) A => ith_default unit_Heading unit_Tuple b m) in
-          let proj2 := eval simpl in
-          (fun b : ilist (@Tuple) A => ith_default unit_Heading unit_Tuple b n)
-            in evar (G : @Tuple (nth_default unit_Heading A m)
-                         -> @Tuple (nth_default unit_Heading A n)
-                         -> C);
-             assert (H : forall p,
-                           f p = G (proj1 p) (proj2 p)) by
-              ( subst G; intro p;
-               let p1 := eval simpl in (proj1 p) in
-               let p2 := eval simpl in (proj2 p) in
-               pattern p1, p2;
-                 match goal with
-                   | [ |- (fun t t' => @?f t t' = @?g t t') _ _ ] => equate f g; reflexivity
-                 end); clear H;
-             let G' := eval unfold G in G in clear G; k G'
-      end.
-
- (* Build pairs of fields + their values. *)
-    Ltac findGoodTerm_dep SC F k :=
-  match F with
-  | fun (a : ?T) b => ?[@?f a b] =>
-    match type of f with
-    | forall a b, {@?X a = _!?fd} + {_} => k (fd, X) (fun _ : @Tuple SC => true)
-    | forall a b, {_!?fd = @?X a} + {_} => k (fd, X) (fun _ : @Tuple SC => true)
-    | forall a b, {@?X a = _``?fd} + {_} => k (fd, X) (fun _ : @Tuple SC => true)
-    | forall a b, {_``?fd = @?X a} + {_} => k (fd, X) (fun _ : @Tuple SC => true)
-    end
-  | fun (a : ?T) b => (@?f a b) && (@?g a b) =>
-    findGoodTerm_dep SC f ltac:(fun fds1 tail1 =>
-      findGoodTerm_dep SC g ltac:(fun fds2 tail2 =>
-        k (fds1, fds2) (fun tup : @Tuple SC => (tail1 tup) && (tail2 tup))))
-  | _ => k tt F
-  end.
-
-    (* Build search a search term from the list of attribute + value pairs in fs. *)
-Ltac createTerm_dep dom fs f fds tail k :=
-  match fs with
-  | nil =>
-    k (fun x : dom => tail)
-  | ?s :: ?fs' =>
-    createTerm_dep dom fs' f fds tail
-      ltac:(fun rest =>
-               findMatchingTerm fds s
-                   ltac:(fun X =>
-                           k (fun x : dom => (Some (X x), rest x)))
-                          || k (fun x : dom => (@None (f s), rest x)))
-  end.
-
-(* Get the heading of [SC] before building the search term. *)
-Ltac makeTerm_dep dom fs SC fds tail k :=
-  match eval hnf in SC with
-  | Build_Heading ?f =>
-    createTerm_dep dom fs f fds tail k
-  end.
-
-Definition Dep_SearchTerm_Wrapper {A} {heading}
-           (search_term_dep : @Tuple heading -> A)
-           (tup : @Tuple heading) : A := search_term_dep tup.
-
-Ltac find_simple_search_term_dep qs_schema idx dom filter_dec search_term :=
-  match type of search_term with
-    | ?dom -> BuildIndexSearchTerm ?attr =>
-      let SC := constr:(QSGetNRelSchemaHeading qs_schema idx) in
-      findGoodTerm_dep SC filter_dec
-                       ltac:(fun fds tail =>
-                               let tail := eval simpl in tail in
-                                   makeTerm_dep dom attr SC fds tail
-                                                ltac:(fun tm => pose tm;
-                                                      (* unification fails if I don't pose tm first... *)
-                                                      unify (Dep_SearchTerm_Wrapper tm) search_term;
-                                                      unfold ExtensionalEq, MatchIndexSearchTerm;
-                                                      simpl; intros;
-                                                      try prove_extensional_eq))
-  end.
-
-(* Find the name of a schema [schemas] with the same heading as [heading] *)
-
-Ltac find_equivalent_tuple schemas heading k :=
-  match schemas with
-    | nil => fail
-    | ?sch' :: ?schemas' =>
-      (let H := fresh in
-       assert (schemaHeading (relSchema sch') = heading) as H
-           by reflexivity;
-       clear H;  k (relName sch'))
-        || find_equivalent_tuple schemas' heading k
-  end.
-
-Ltac find_equivalent_search_term_pair m n build_search_term_dep :=
-match goal with
-    [ H : @DelegateToBag_AbsR ?qs_schema ?indices ?r_o ?r_n
-      |- ExtensionalEq ?f _ ] =>
-    get_ithDefault_pair f m n
-      ltac:(fun filter_dec =>
-        let dom := match type of filter_dec with
-                     | ?A -> ?B -> bool => constr:(A)
-                   end in
-        let heading := match type of filter_dec with
-                         | ?A -> @Tuple ?heading -> bool => constr:(heading)
-                       end in
-        let schemas := eval simpl in (qschemaSchemas qs_schema) in
-            find_equivalent_tuple schemas heading
-              ltac:(fun id => let idx' := constr:({| bindex := id |} : BoundedIndex (map relName (qschemaSchemas qs_schema)))
-                              in let idx := eval simpl in idx' in
-    let idx_search_update_term := eval simpl in (ith_Bounded relName indices idx) in
-    let search_term_type := eval simpl in (BagSearchTermType idx_search_update_term) in
-        let search_term_matcher := eval simpl in (BagMatchSearchTerm idx_search_update_term) in
-        makeEvar (dom -> search_term_type)
-                 ltac: (fun search_term =>
-                          let eqv := fresh in
-                          assert (forall a b, filter_dec a b
-                                                = search_term_matcher (search_term a) b) as eqv;
-                        [ build_search_term_dep qs_schema idx
-                          dom filter_dec search_term
-                        | match goal with
-                            |- ExtensionalEq ?f ?search_term' =>
-                            match type of f with
-                                | ?A -> _ =>
-                                  unify search_term' (fun a : A => search_term_matcher (search_term (ith_default unit_Heading unit_Tuple a m))
-            ((ith_default unit_Heading unit_Tuple a n)))
-                            end
-                                                  end;
-                          unfold ExtensionalEq in *; intros;
-                          simpl in *; rewrite eqv; reflexivity
-]))) end.
-
-Ltac find_equivalent_search_term m build_search_term :=
-match goal with
-    [ H : @DelegateToBag_AbsR ?qs_schema ?indices ?r_o ?r_n
-      |- ExtensionalEq ?f _ ] =>
-    get_ithDefault f m
-      ltac:(fun filter_dec =>
-        let heading := match type of filter_dec with
-                         | @Tuple ?heading -> bool => constr:(heading)
-                       end in
-        let schemas := eval simpl in (qschemaSchemas qs_schema) in
-            find_equivalent_tuple schemas heading
-              ltac:(fun id => let idx' := constr:({| bindex := id |} : BoundedIndex (map relName (qschemaSchemas qs_schema)))
-                              in let idx := eval simpl in idx' in
-    let idx_search_update_term := eval simpl in (ith_Bounded relName indices idx) in
-    let search_term_type := eval simpl in (BagSearchTermType idx_search_update_term) in
-        let search_term_matcher := eval simpl in (BagMatchSearchTerm idx_search_update_term) in
-        makeEvar (search_term_type)
-                 ltac: (fun search_term =>
-                          let eqv := fresh in
-                          assert (forall a, filter_dec a
-                                                = search_term_matcher search_term a) as eqv;
-                        [ build_search_term qs_schema idx
-                          filter_dec search_term
-                        | match goal with
-                              |- ExtensionalEq ?f ?search_term' =>
-                              match type of f with
-                                | ?A -> _ =>
-                                  unify search_term' (fun a : A => search_term_matcher search_term (ith_default unit_Heading unit_Tuple a m))
-                              end
-                          end;
-                          unfold ExtensionalEq in *; intros;
-                          simpl in *; rewrite eqv; reflexivity
-]))) end.
-
-Corollary refine_Join_Lists_filter_filter_search_term_snd_dep'
-          qs_schema BagIndexKeys
-        (ResultT : Type) :
-    forall (r_n : IndexedQueryStructure qs_schema BagIndexKeys)
-           idx idx'
-           (search_pattern : _ -> _)
-           (resultComp : ilist (@Tuple) [_; _] -> Comp (list ResultT))
-           filter_rest st,
-      refine (cl <- CallBagMethod idx {| bindex := "Find" |} r_n st;
-              l' <- (Join_Lists (Build_single_Tuple_list (snd cl))
-                                (fun _ => l <- CallBagMethod idx' {| bindex := "Enumerate" |} r_n ();
-                                 ret (snd l)));
-              List_Query_In (filter (fun a : ilist (@Tuple) [_ ; _] => BagMatchSearchTerm _ (search_pattern (ilist_tl a)) (ilist_hd a) && filter_rest a) l')
-                            resultComp)
-             (cl <- CallBagMethod idx {| bindex := "Find" |} r_n st;
-              l' <- (Join_Lists (Build_single_Tuple_list (snd cl))
-                                (fun tup => l <- CallBagMethod idx' {| bindex := "Find" |} r_n (search_pattern tup);
-                                             ret (snd l)));
-                      List_Query_In (filter filter_rest l') resultComp).
-  Proof.
-    intros; f_equiv; intro;
-    apply refine_Join_Lists_filter_search_term_snd_dep.
-  Qed.
-
-  Ltac convert_filter_to_find':=
-    try match goal with
-            |- context[filter (fun a => (_ && _) && true) _] =>
-            setoid_rewrite <- andb_assoc; simpl
-        end;
-    match goal with
-      | H : @DelegateToBag_AbsR ?qs_schema ?indices ?r_o ?r_n
-        |- context[l <- CallBagMethod ?idx ``("Enumerate") ?r_n ();
-                    List_Query_In (filter (fun a => MatchIndexSearchTerm ?st (ilist_hd a) && @?filter_rest a)
-                                          (Build_single_Tuple_list (snd l))) ?resultComp] =>
-        let b := fresh in
-        pose proof (@refine_Query_For_In_Find_single _ _ _ r_o r_n H idx st resultComp filter_rest) as b;
-          simpl in b; setoid_rewrite b; clear b
-
-      | H : @DelegateToBag_AbsR ?qs_schema ?indices ?r_o ?r_n
-        |- context[l <- CallBagMethod ?idx ``("Enumerate") ?r_n ();
-                    l' <- Join_Lists (Build_single_Tuple_list (snd l)) ?cl;
-                    List_Query_In (filter (fun a => MatchIndexSearchTerm ?st (ilist_hd (ilist_tl a)) && @?filter_rest a)
-                                          l') ?resultComp] =>
-        let b := fresh in
-        pose proof (fun foo => @refine_Join_Lists_filter_search_term_fst _ _ _ r_n idx _ cl st resultComp foo filter_rest) as b;
-          simpl in b; setoid_rewrite b;
-          [ clear b
-          | match goal with
-              | |- context [CallBagMethod ?idx' ``("Enumerate") _ _] =>
-                intros; eapply (realizeable_Enumerate (r_o := r_o) (r_n := r_n) idx' H)
-              | |- context [CallBagMethod ?idx' ``("Find") _ _] =>
-                intros; eapply (realizeable_Find (r_o := r_o) (r_n := r_n) idx' H)
-            end]
-      | H : @DelegateToBag_AbsR ?qs_schema ?indices ?r_o ?r_n
-        |- context[l <- CallBagMethod ?idx ``("Find") ?r_n ?st;
-                    l' <- Join_Lists (Build_single_Tuple_list (snd l))
-                       (fun _ : ilist (@Tuple) [?heading] =>
-                          l <- CallBagMethod ?idx' ``("Enumerate") ?r_n ();
-                        ret (snd l));
-                    List_Query_In (filter (fun a => MatchIndexSearchTerm (Dep_SearchTerm_Wrapper ?st' (ilist_hd (ilist_tl a)))
-                                                                         (ilist_hd a) && @?filter_rest a) l') ?resultComp] =>
-        let b := fresh in
-        pose proof (@refine_Join_Lists_filter_filter_search_term_snd_dep' _ _ _ r_n idx idx'
-                                                                          (fun a => Dep_SearchTerm_Wrapper st' (ilist_hd a))
-                                                                          resultComp filter_rest st) as b;
-          unfold Dep_SearchTerm_Wrapper in b; simpl in b; setoid_rewrite b; clear b
-      (* The final case replaces the last filter and the Return statement. *)
-      | _ => setoid_rewrite filter_true; setoid_rewrite refine_List_Query_In_Return
-    end.
-
-  Ltac convert_filter_to_find :=
-    simpl; repeat convert_filter_to_find'.
-
-  (* This also implements Fors *)
-  Ltac Implement_Aggregates :=
-    repeat
-      match goal with
-        | |- context[For _] => setoid_rewrite refine_For_List
-        | |- context[Count _] => setoid_rewrite refine_Count
-      end.
-
-  (* Commits the database at the end of a method call. *)
-  Ltac commit :=
-    match goal with
-      | [H : @DelegateToBag_AbsR ?qs_schema ?indices ?r_o ?r_n
-         |- context[{r_n' : IndexedQueryStructure ?qs_schema ?indices | DelegateToBag_AbsR ?r_o r_n'}] ]
-        => setoid_rewrite (refine_pick_val (@DelegateToBag_AbsR qs_schema indices r_o) H);
-          simplify with monad laws
-    end.
 
 Theorem BookStoreManual :
   Sharpened BookStoreSpec.
@@ -769,835 +202,6 @@ Proof.
 
   (* At this point our implementation is fully computational: we're done! *)
 
-  Require Import ADTNotation.BuildComputationalADT.
-  Require Import ADT.ComputationalADT.
-
-  Ltac FullySharpenEachMethod delegateSigs delegateSpecs cRep' cAbsR' :=
-    match goal with
-      |- Sharpened (@BuildADT ?Rep ?consSigs ?methSigs ?consDefs ?methDefs) => 
-      ilist_of_evar
-        (ilist (fun nadt => ComputationalADT.cADT (namedADTSig nadt)) delegateSigs)
-        (fun DelegateImpl Sig => ComputationalADT.cMethodType (cRep' DelegateImpl) (methDom Sig) (methCod Sig))
-        methSigs
-        ltac:(fun cMeths => 
-                ilist_of_evar
-                  (ilist (fun nadt => ComputationalADT.cADT (namedADTSig nadt)) delegateSigs)
-                  (fun DelegateImpl Sig => ComputationalADT.cConstructorType (cRep' DelegateImpl) (consDom Sig))
-                  consSigs
-                  ltac:(fun cCons =>  
-                          eapply
-                            (@Notation_Friendly_SharpenFully
-                               _ 
-                               consSigs
-                               methSigs
-                               consDefs
-                               methDefs
-                               delegateSigs
-                               cRep'
-                               cCons
-                               cMeths
-                               delegateSpecs
-                               cAbsR')));
-        unfold Dep_Type_BoundedIndex_app_comm_cons
-    end; simpl; split.
-
-  Fixpoint Build_IndexedQueryStructure_Impl_Sigs
-    {indices : list NamedSchema}
-      (Index : ilist (fun ns : NamedSchema => SearchUpdateTerms (schemaHeading (relSchema ns))) indices)
-    : list NamedADTSig :=
-    match indices as indices return ilist _ indices -> list NamedADTSig with
-      | nil => fun _ => nil
-      | cons ns indices' =>
-        fun Index =>
-          {| ADTSigname := relName ns;
-             namedADTSig := 
-               BagSig (@Tuple (schemaHeading (relSchema ns))) (BagSearchTermType (ilist_hd Index)) (BagUpdateTermType (ilist_hd Index)) |}
-                       :: @Build_IndexedQueryStructure_Impl_Sigs indices' (ilist_tl Index)
-    end Index.
-
-  Fixpoint Build_IndexedQueryStructure_Impl_Specs
-           {indices : list NamedSchema}
-           (Index : ilist (fun ns : NamedSchema => SearchUpdateTerms (schemaHeading (relSchema ns))) indices)
-  : ilist (fun ns => ADT (namedADTSig ns)) (@Build_IndexedQueryStructure_Impl_Sigs indices Index) :=
-    match indices as indices return
-          forall (Index : ilist _ indices),
-            ilist (fun ns : NamedADTSig => ADT (namedADTSig ns))
-                  (@Build_IndexedQueryStructure_Impl_Sigs indices Index)
-    with
-      | nil => fun _ => inil _
-      | cons ns indices' =>
-        fun Index => icons {| ADTSigname := relName ns;
-                              namedADTSig := _ |}
-                           (@BagSpec (@Tuple (schemaHeading (relSchema ns)))
-                                     (BagSearchTermType (ilist_hd Index))
-                                     (BagUpdateTermType (ilist_hd Index))
-                                     (BagMatchSearchTerm (ilist_hd Index))
-                                     (BagApplyUpdateTerm (ilist_hd Index)))
-                           (@Build_IndexedQueryStructure_Impl_Specs indices' (ilist_tl Index))
-    end Index.
-  
-  Definition Build_IndexedQueryStructure_Impl_cRep
-           {indices : list NamedSchema}
-           (Index : ilist (fun ns : NamedSchema => SearchUpdateTerms (schemaHeading (relSchema ns))) indices)
-           (DelegateImpls : ilist (fun ns => cADT (namedADTSig ns)) (@Build_IndexedQueryStructure_Impl_Sigs indices Index))
-  : Type
-    :=
-    i2list
-      (fun (ns : NamedADTSig)
-           (index : cADT (namedADTSig ns)) => cRep index) DelegateImpls.
-
-  Fixpoint map_IndexedQS_idx_boundi
-        {indices}
-  : forall
-      n
-      (Index : ilist
-                 (fun ns : NamedSchema =>
-                    SearchUpdateTerms (schemaHeading (relSchema ns)))
-                 indices)
-      idx, 
-      nth_error
-        (map ADTSigname (Build_IndexedQueryStructure_Impl_Sigs Index))
-        n = Some idx
-      ->  nth_error (map relName indices) n = Some idx.
-  Proof.
-    refine (match indices with
-              | nil => _
-              | ns :: indices' =>
-                fun n => 
-                  match n return
-                        forall
-                          (Index : ilist
-                                     (fun ns : NamedSchema =>
-                                        SearchUpdateTerms (schemaHeading (relSchema ns)))
-                                     (ns :: indices'))
-                          idx,
-                          nth_error (map ADTSigname (Build_IndexedQueryStructure_Impl_Sigs Index)) n =
-                          Some idx ->
-                          nth_error (map relName (ns :: indices')) n = Some idx
-                  with
-                    | 0 => fun Index idx nth_n => nth_n
-                    | S n' => fun Index => (map_IndexedQS_idx_boundi indices' n' (ilist_tl Index))
-                  end
-            end);
-    simpl; intros; try discriminate; eauto.
-  Defined.
-  
-  Definition map_IndexedQS_idx
-             indices
-             (Index : ilist (fun ns : NamedSchema => SearchUpdateTerms (schemaHeading (relSchema ns))) indices )
-             (idx : BoundedIndex
-                      (map ADTSigname
-                           (Build_IndexedQueryStructure_Impl_Sigs Index)))
-  : BoundedIndex (map relName indices) := 
-    {| bindex := bindex idx;
-       indexb := {| ibound := ibound (indexb idx);
-                    boundi := map_IndexedQS_idx_boundi _ Index (boundi (indexb idx))|} |}.
-
-  Fixpoint map_IndexedQS_idx_boundi'
-        {indices}
-  : forall
-      n
-      (Index : ilist
-                 (fun ns : NamedSchema =>
-                    SearchUpdateTerms (schemaHeading (relSchema ns)))
-                 indices)
-      idx, 
-      nth_error (map relName indices) n = Some idx
-      -> nth_error
-        (map ADTSigname (Build_IndexedQueryStructure_Impl_Sigs Index))
-        n = Some idx.
-  Proof.
-    refine (match indices with
-              | nil => _
-              | ns :: indices' =>
-                fun n => 
-                  match n return
-                        forall
-                          (Index : ilist
-                                     (fun ns : NamedSchema =>
-                                        SearchUpdateTerms (schemaHeading (relSchema ns)))
-                                     (ns :: indices'))
-                          idx,
-                          nth_error (map relName (ns :: indices')) n = Some idx
-                          -> nth_error (map ADTSigname (Build_IndexedQueryStructure_Impl_Sigs Index)) n = Some idx
-                  with
-                    | 0 => fun Index idx nth_n => nth_n
-                    | S n' => fun Index => (map_IndexedQS_idx_boundi' indices' n' (ilist_tl Index))
-                  end
-            end);
-    simpl; intros; try discriminate; eauto.
-  Defined.
-  
-  Definition map_IndexedQS_idx'
-             indices
-             (Index : ilist (fun ns : NamedSchema => SearchUpdateTerms (schemaHeading (relSchema ns))) indices )
-             (idx : BoundedIndex (map relName indices))
-  : BoundedIndex
-                      (map ADTSigname
-                           (Build_IndexedQueryStructure_Impl_Sigs Index)) := 
-    {| bindex := bindex idx;
-       indexb := {| ibound := ibound (indexb idx);
-                    boundi := map_IndexedQS_idx_boundi' _ Index (boundi (indexb idx))|} |}.
-
-  Lemma ith_Build_IndexedQueryStructure_Impl_Sigs_eq
-        {indices}
-  : forall
-      (Index : ilist (fun ns : NamedSchema => SearchUpdateTerms (schemaHeading (relSchema ns))) indices )
-      (idx : BoundedIndex
-               (map ADTSigname
-                    (Build_IndexedQueryStructure_Impl_Sigs Index))),
-      (BagSig (@Tuple (schemaHeading (relSchema ((nth_Bounded relName indices (map_IndexedQS_idx Index idx))))))
-              (BagSearchTermType
-                 (ith_Bounded relName Index (map_IndexedQS_idx Index idx)))
-              (BagUpdateTermType
-                 (ith_Bounded relName Index (map_IndexedQS_idx Index idx))))
-      = namedADTSig
-          (nth_Bounded ADTSigname (Build_IndexedQueryStructure_Impl_Sigs Index) idx).
-  Proof.
-    destruct idx as [idx [n nth_n]].
-    revert Index idx n nth_n.
-    induction indices; destruct n; simpl; intros; try discriminate; eauto.
-    eapply (IHindices (ilist_tl Index) idx n nth_n).
-  Defined.
-
-  Lemma ith_Build_IndexedQueryStructure_Impl_Specs_eq
-        {indices}
-  : forall
-      (Index : ilist (fun ns : NamedSchema => SearchUpdateTerms (schemaHeading (relSchema ns))) indices )
-      (idx : BoundedIndex
-               (map ADTSigname
-                    (Build_IndexedQueryStructure_Impl_Sigs Index))),
-      ith_Bounded ADTSigname (Build_IndexedQueryStructure_Impl_Specs Index) idx = 
-  eq_rect _ ADT
-          (@BagSpec (@Tuple (schemaHeading (relSchema (@nth_Bounded NamedSchema string relName
-                                                                    indices (map_IndexedQS_idx Index idx)))))
-                    (BagSearchTermType (ith_Bounded _ Index (map_IndexedQS_idx Index idx)))
-                    (BagUpdateTermType (ith_Bounded _ Index (map_IndexedQS_idx Index idx)))
-                    (BagMatchSearchTerm (ith_Bounded _ Index (map_IndexedQS_idx Index idx)))
-                    (BagApplyUpdateTerm (ith_Bounded _ Index (map_IndexedQS_idx Index idx))))
-                    _ (ith_Build_IndexedQueryStructure_Impl_Sigs_eq Index idx).
-  Proof.
-    destruct idx as [idx [n nth_n]].
-    revert Index idx n nth_n.
-    induction indices; destruct n; simpl; intros; try discriminate; eauto.
-    eapply (IHindices (ilist_tl Index) idx n nth_n).
-  Defined.
-        
-  Definition map_IndexedQS_Rep 
-             {indices}
-             (Index : ilist (fun ns : NamedSchema => SearchUpdateTerms (schemaHeading (relSchema ns))) indices )
-             idx
-             (rep : @IndexedEnsemble
-                      (@Tuple
-                         (schemaHeading
-                            (relSchema
-                               (@nth_Bounded NamedSchema string relName
-                                             indices (map_IndexedQS_idx Index idx) )))))
-  : Rep
-      (ith_Bounded ADTSigname
-                   (Build_IndexedQueryStructure_Impl_Specs Index) idx).
-  Proof.
-    destruct idx as [idx [n nth_n]].
-    revert Index idx n nth_n rep.
-    induction indices; destruct n; simpl; intros; try discriminate; eauto.
-    eapply IHindices; eauto.
-  Defined.
-
-  Definition map_IndexedQS_Rep'
-             {indices}
-             (Index : ilist (fun ns : NamedSchema => SearchUpdateTerms (schemaHeading (relSchema ns))) indices )
-             idx
-             (rep : Rep
-                      (ith_Bounded ADTSigname
-                                   (Build_IndexedQueryStructure_Impl_Specs Index)
-                                   (map_IndexedQS_idx' Index idx)))
-  : @IndexedEnsemble
-      (@Tuple
-         (schemaHeading
-            (relSchema
-               (@nth_Bounded NamedSchema string relName
-                             indices idx )))).
-  Proof.
-    destruct idx as [idx [n nth_n]].
-    revert Index idx n nth_n rep.
-    induction indices; destruct n; simpl; intros; try discriminate; eauto.
-    eapply (IHindices (ilist_tl Index)); eauto.
-  Defined.
-    
-  Definition Build_IndexedQueryStructure_Impl_AbsR
-             {qs_schema : QueryStructureSchema}
-             (Index : ilist (fun ns : NamedSchema => SearchUpdateTerms (schemaHeading (relSchema ns))) (qschemaSchemas qs_schema) )
-             (DelegateImpls : ilist (fun ns => cADT (namedADTSig ns))
-                                     (Build_IndexedQueryStructure_Impl_Sigs Index))
-             (ValidImpl :
-                forall idx,
-                  refineADT (ith_Bounded ADTSigname
-                                         (Build_IndexedQueryStructure_Impl_Specs Index) idx)
-                            (LiftcADT (ith_Bounded ADTSigname DelegateImpls idx)))
-             (r_o : IndexedQueryStructure qs_schema Index)
-             (r_n : Build_IndexedQueryStructure_Impl_cRep Index DelegateImpls)
-  : Prop := 
-    forall idx,
-      AbsR (ValidImpl idx)
-           (map_IndexedQS_Rep Index idx (GetIndexedRelation r_o (map_IndexedQS_idx Index idx)))
-           (i2th_Bounded ADTSigname r_n idx).
-
-  Definition map_IndexedQS_Rep''
-             {indices}
-             (Index : ilist (fun ns : NamedSchema => SearchUpdateTerms (schemaHeading (relSchema ns))) indices )
-             idx
-             (rep : @IndexedEnsemble
-                      (@Tuple
-                         (schemaHeading
-                            (relSchema
-                               (@nth_Bounded NamedSchema string relName
-                                             indices idx)))))
-  : Rep
-      (ith_Bounded ADTSigname
-                   (Build_IndexedQueryStructure_Impl_Specs Index) (map_IndexedQS_idx' Index idx)).
-  Proof.
-    destruct idx as [idx [n nth_n]].
-    revert Index idx n nth_n rep.
-    induction indices; destruct n; simpl; intros; try discriminate; eauto.
-    eapply IHindices; eauto.
-  Defined.
-
-  Definition Build_IndexedQueryStructure_Impl_AbsR''
-             {qs_schema : QueryStructureSchema}
-             (Index : ilist (fun ns : NamedSchema => SearchUpdateTerms (schemaHeading (relSchema ns))) (qschemaSchemas qs_schema) )
-             (DelegateImpls : ilist (fun ns => cADT (namedADTSig ns))
-                                     (Build_IndexedQueryStructure_Impl_Sigs Index))
-             (ValidImpl :
-                forall idx : BoundedIndex (map relName (qschemaSchemas qs_schema)),
-                  refineADT (ith_Bounded ADTSigname
-                                         (Build_IndexedQueryStructure_Impl_Specs Index) (map_IndexedQS_idx' Index idx))
-                            (LiftcADT (ith_Bounded ADTSigname DelegateImpls (map_IndexedQS_idx' Index idx))))
-             (r_o : IndexedQueryStructure qs_schema Index)
-             (r_n : Build_IndexedQueryStructure_Impl_cRep Index DelegateImpls)
-  : Prop := 
-    forall idx,
-      AbsR (ValidImpl idx)
-           (map_IndexedQS_Rep'' Index idx (GetIndexedRelation r_o idx))
-           (i2th_Bounded ADTSigname r_n (map_IndexedQS_idx' Index idx)).
-
-  Definition CallBagImplMethod
-             {qs_schema : QueryStructureSchema}
-             (Index : ilist (fun ns : NamedSchema => SearchUpdateTerms (schemaHeading (relSchema ns))) (qschemaSchemas qs_schema) )
-             (DelegateImpls : ilist (fun ns => cADT (namedADTSig ns))
-                                    (Build_IndexedQueryStructure_Impl_Sigs Index))
-             idx midx
-             (r_n : Build_IndexedQueryStructure_Impl_cRep Index DelegateImpls) :=
-    cMethods (ith_Bounded ADTSigname DelegateImpls idx) midx (i2th_Bounded _ r_n idx).
-
-  Definition CallBagImplConstructor
-             {qs_schema : QueryStructureSchema}
-             (Index : ilist (fun ns : NamedSchema => SearchUpdateTerms (schemaHeading (relSchema ns))) (qschemaSchemas qs_schema) )
-             (DelegateImpls : ilist (fun ns => cADT (namedADTSig ns))
-                                    (Build_IndexedQueryStructure_Impl_Sigs Index))
-             idx midx :=
-    cConstructors (ith_Bounded ADTSigname DelegateImpls idx) midx .
-
-  Fixpoint Build_IndexedQueryStructure_Impl_midx
-           {indices}
-           (P : ADTSig -> Type)
-  : forall (Index : ilist (fun ns : NamedSchema => SearchUpdateTerms (schemaHeading (relSchema ns))) indices)
-             ridx
-             (midx : P
-                       (BagSig (@Tuple (schemaHeading
-                            (relSchema
-                               (@nth_Bounded NamedSchema string relName
-                                             indices (map_IndexedQS_idx Index ridx ) ))))
-                               (BagSearchTermType
-                                  (ith_Bounded relName Index (map_IndexedQS_idx Index ridx)))
-                               (BagUpdateTermType
-                                  (ith_Bounded relName Index (map_IndexedQS_idx Index ridx))))),
-      P
-        (namedADTSig
-           (nth_Bounded ADTSigname (Build_IndexedQueryStructure_Impl_Sigs Index)
-                        ridx)) := 
-    match indices return
-          forall (Index : ilist
-                            (fun ns : NamedSchema =>
-                               SearchUpdateTerms (schemaHeading (relSchema ns)))
-                            indices)
-                 (ridx : BoundedIndex
-                           (map ADTSigname (Build_IndexedQueryStructure_Impl_Sigs Index)))
-                 (midx : P
-                       (BagSig (@Tuple (schemaHeading
-                            (relSchema
-                               (@nth_Bounded NamedSchema string relName
-                                             indices (map_IndexedQS_idx Index ridx ) ))))
-                               (BagSearchTermType
-                                  (ith_Bounded relName Index (map_IndexedQS_idx Index ridx)))
-                               (BagUpdateTermType
-                                  (ith_Bounded relName Index (map_IndexedQS_idx Index ridx))))),
-      P
-        (namedADTSig
-           (nth_Bounded ADTSigname (Build_IndexedQueryStructure_Impl_Sigs Index)
-                        ridx))
-    with
-      | nil => fun _ ridx => BoundedIndex_nil _ ridx
-      | ns :: indices' =>
-        fun Index ridx =>  
-          match ridx with
-            | {| bindex := ridx;
-                 indexb := {|ibound := n;
-                             boundi := nth_n |}|} => 
-              match n return
-                    forall
-                      (Index' : ilist
-                                  (fun ns : NamedSchema =>
-                                     SearchUpdateTerms (schemaHeading (relSchema ns))) (ns :: indices'))
-                      ridx nth_n,
-                      let idx := {| bindex := ridx;
-                                    indexb := {|ibound := n;
-                                                boundi := nth_n |}|} in 
-                      P
-                                (BagSig (@Tuple (schemaHeading
-                                                   (relSchema
-                                                      (@nth_Bounded NamedSchema string relName
-                                                                    (ns :: indices') (map_IndexedQS_idx Index' idx ) ))))
-                                        (BagSearchTermType
-                                           (ith_Bounded relName Index' (map_IndexedQS_idx Index' idx)))
-                                        (BagUpdateTermType
-                                           (ith_Bounded relName Index' (map_IndexedQS_idx Index' idx)))) -> 
-                      P
-                        (namedADTSig
-                           (nth_Bounded ADTSigname (Build_IndexedQueryStructure_Impl_Sigs Index')
-                                        {| bindex := ridx;
-                                           indexb := {|ibound := n;
-                                                       boundi := nth_n |}|}))
-              with
-                | 0 => fun Index idx nth_n midx => midx
-                | S n' => fun Index idx nth_n midx =>
-                            (@Build_IndexedQueryStructure_Impl_midx
-                               indices' P (ilist_tl Index)
-                               {| bindex := idx;
-                                  indexb := {|ibound := n';
-                                              boundi := nth_n |}|}
-                               midx)
-              end Index ridx nth_n 
-                            end
-         end.  
-
-
-(*fst
-    (MethodDomCod
-       (BagSig Tuple (BagSearchTermType (ith_Bounded relName Index ridx))
-          (BagUpdateTermType (ith_Bounded relName Index ridx))) midx)"
- while it is expected to have type
- "fst
-    (MethodDomCod
-       (namedADTSig
-          (nth_Bounded ADTSigname
-             (Build_IndexedQueryStructure_Impl_Sigs Index) ridx')) midx')" *)
-  
-  Definition Build_IndexedQueryStructure_Impl_MethodDom
-           {indices}
-  : forall (Index : ilist (fun ns : NamedSchema => SearchUpdateTerms (schemaHeading (relSchema ns))) indices)
-           ridx
-           midx,
-      fst (MethodDomCod
-             (BagSig (@Tuple (schemaHeading (relSchema (nth_Bounded relName indices  ridx))))
-                     (BagSearchTermType
-                        (ith_Bounded relName Index ridx))
-                     (BagUpdateTermType
-                        (ith_Bounded relName Index ridx)))
-             midx)
-    -> fst
-        (MethodDomCod
-           (namedADTSig
-              (nth_Bounded ADTSigname
-                           (Build_IndexedQueryStructure_Impl_Sigs Index) (map_IndexedQS_idx' Index ridx)))
-           (Build_IndexedQueryStructure_Impl_midx MethodIndex Index (map_IndexedQS_idx' Index ridx) midx)).
-  Proof.
-    destruct ridx as [idx [n nth_n]]; revert Index idx n nth_n.
-    induction indices.
-  - destruct n; simpl; discriminate.
-  - destruct n; simpl; eauto.
-    intros; eapply (IHindices (ilist_tl Index) idx n nth_n); eauto.
-  Defined.
-
-  Definition Build_IndexedQueryStructure_Impl_MethodCod
-           {indices}
-  : forall (Index : ilist (fun ns : NamedSchema => SearchUpdateTerms (schemaHeading (relSchema ns))) indices)
-           ridx
-           midx,
-      snd
-        (MethodDomCod
-           (namedADTSig
-              (nth_Bounded ADTSigname
-                           (Build_IndexedQueryStructure_Impl_Sigs Index) (map_IndexedQS_idx' Index ridx)))
-           (Build_IndexedQueryStructure_Impl_midx MethodIndex Index (map_IndexedQS_idx' Index ridx) midx))
-  ->       snd (MethodDomCod
-             (BagSig (@Tuple (schemaHeading (relSchema (nth_Bounded relName indices  ridx))))
-                     (BagSearchTermType
-                        (ith_Bounded relName Index ridx))
-                     (BagUpdateTermType
-                        (ith_Bounded relName Index ridx)))
-             midx)
-.
-  Proof.
-    destruct ridx as [idx [n nth_n]]; revert Index idx n nth_n.
-    induction indices.
-  - destruct n; simpl; discriminate.
-  - destruct n; simpl; eauto.
-    intros; eapply (IHindices (ilist_tl Index) idx n nth_n); eauto.
-  Defined.
-
-Lemma ith_Build_IndexedQueryStructure_Impl_Methods
-        {indices}
-  : forall
-      (Index : ilist (fun ns : NamedSchema => SearchUpdateTerms (schemaHeading (relSchema ns))) indices )
-      (idx : BoundedIndex
-               (map ADTSigname
-                    (Build_IndexedQueryStructure_Impl_Sigs Index))),
-      Methods (ith_Bounded ADTSigname (Build_IndexedQueryStructure_Impl_Specs Index) idx) = 
-      eq_rect _ (fun r => forall idx, methodType (Rep r) _ _ )
-              (Methods (eq_rect _ ADT
-                                (@BagSpec (@Tuple (schemaHeading (relSchema (@nth_Bounded NamedSchema string relName
-                                                                                          indices (map_IndexedQS_idx Index idx)))))
-                                          (BagSearchTermType (ith_Bounded _ Index (map_IndexedQS_idx Index idx)))
-                                          (BagUpdateTermType (ith_Bounded _ Index (map_IndexedQS_idx Index idx)))
-                                          (BagMatchSearchTerm (ith_Bounded _ Index (map_IndexedQS_idx Index idx)))
-                                          (BagApplyUpdateTerm (ith_Bounded _ Index (map_IndexedQS_idx Index idx))))
-                                _ (ith_Build_IndexedQueryStructure_Impl_Sigs_eq Index idx)))
-              _ (eq_sym (ith_Build_IndexedQueryStructure_Impl_Specs_eq Index idx)).
-  Proof.
-    destruct idx as [idx [n nth_n]].
-    revert Index idx n nth_n.
-    induction indices; destruct n; simpl; intros; try discriminate; eauto.
-    eapply (IHindices (ilist_tl Index) idx n nth_n).
-  Defined.
-  
-  Lemma refine_Mapped_Methods
-        {indices}
-        (Index : ilist (fun ns : NamedSchema => SearchUpdateTerms (schemaHeading (relSchema ns))) (indices) )
-  :  forall
-      ridx,
-      forall
-        (r_o : @IndexedEnsemble (@Tuple (schemaHeading (relSchema (nth_Bounded relName indices ridx)))))
-      midx 
-      d r s,
-        let ridx' := map_IndexedQS_idx' Index ridx in 
-        let midx' := Build_IndexedQueryStructure_Impl_midx MethodIndex Index ridx' midx in
-        let d' := Build_IndexedQueryStructure_Impl_MethodDom Index ridx _ d in
-Methods
-     (ith_Bounded ADTSigname (Build_IndexedQueryStructure_Impl_Specs Index) ridx') midx'
-     (map_IndexedQS_Rep'' Index ridx r_o) d'
-     ↝ (r, s) ->
-Methods
-  (BagSpec (BagMatchSearchTerm (ith_Bounded relName Index ridx))
-           (BagApplyUpdateTerm (ith_Bounded relName Index ridx))) midx r_o d
-   ↝ (map_IndexedQS_Rep' Index ridx r,
-     Build_IndexedQueryStructure_Impl_MethodCod Index ridx midx s).
-  Proof.
-    intros; pose proof (ith_Build_IndexedQueryStructure_Impl_Methods Index ridx') as H';
-    rewrite H' in H; revert H; clear H'.
-    unfold d', midx', ridx' in *; clear ridx' midx' d'.
-    revert r_o d r s.
-    intro; eapply (Iterate_Dep_Type_BoundedIndex_equiv_1) with (idx := midx);
-    simpl.
-    intuition;
-      simpl in *;
-      first [revert midx r_o d r s H
-            | revert midx r_o b a r s H ];
-    try (destruct ridx as [idx [n nth_n]];
-      revert idx n nth_n;
-      unfold IndexedQueryStructure, GetIndexedRelation in *;
-      unfold list_ind, list_rect in *;
-      induction indices; destruct n; simpl; try (intros; discriminate); eauto;
-      eapply IHindices).
-  Qed.
-  
-  Lemma refine_BagImplMethods
-        {qs_schema : QueryStructureSchema}
-        (Index : ilist (fun ns : NamedSchema => SearchUpdateTerms (schemaHeading (relSchema ns))) (qschemaSchemas qs_schema) )
-        (DelegateImpls : ilist (fun ns => cADT (namedADTSig ns))
-                               (Build_IndexedQueryStructure_Impl_Sigs Index))
-        ValidImpl
-  :  forall (r_o : IndexedQueryStructure qs_schema Index)
-            (r_n : Build_IndexedQueryStructure_Impl_cRep Index DelegateImpls)
-            ridx,
-            let ridx' := map_IndexedQS_idx' Index ridx in 
-            forall (midx : MethodIndex
-                     (BagSig Tuple
-                             (BagSearchTermType
-                                (ith_Bounded relName Index (map_IndexedQS_idx Index ridx')))
-                             (BagUpdateTermType
-                                (ith_Bounded relName Index (map_IndexedQS_idx Index ridx')))))
-                   (d : fst
-                          (MethodDomCod
-                             (BagSig (@Tuple (schemaHeading (relSchema (nth_Bounded relName (qschemaSchemas qs_schema) ridx))))
-                                     (BagSearchTermType (ith_Bounded relName Index ridx))
-                                     (BagUpdateTermType (ith_Bounded relName Index ridx))) midx)),
-       let midx' := Build_IndexedQueryStructure_Impl_midx MethodIndex Index ridx' midx in
-       let d' := Build_IndexedQueryStructure_Impl_MethodDom Index ridx _ d in
-       Build_IndexedQueryStructure_Impl_AbsR'' ValidImpl r_o r_n ->
-       exists r_o',
-         AbsR (ValidImpl ridx) r_o' (fst (CallBagImplMethod ridx' midx' r_n d'))
-         /\ refine (CallBagMethod ridx midx r_o d)
-                   (ret (map_IndexedQS_Rep' _ _ r_o',
-                         Build_IndexedQueryStructure_Impl_MethodCod Index ridx _
-                                                                    (snd (CallBagImplMethod (map_IndexedQS_idx' Index ridx) midx' r_n d')))).
-    intros.
-    pose proof (ADTRefinementPreservesMethods (ValidImpl ridx) midx'
-                                              (map_IndexedQS_Rep'' Index ridx
-                                                                 (GetIndexedRelation r_o ridx))
-                                              (i2th_Bounded _ r_n ridx') d' (H ridx) (ReturnComputes _)).
-    Local Arguments map_IndexedQS_Rep : simpl never.
-    inversion_by computes_to_inv; subst.
-    exists (fst x);
-      unfold CallBagImplMethod; simpl in *. 
-      split; simpl.
-      - pose proof (f_equal fst H3) as eq_x0; simpl in eq_x0.
-        rewrite eq_x0 in H2; simpl in H2; apply H2.
-    - pose proof (f_equal snd H3) as eq_x; simpl in eq_x.
-      assert (refine (CallBagMethod ridx midx r_o d)
-                     (ret
-                        (map_IndexedQS_Rep' Index ridx (fst x),
-                         Build_IndexedQueryStructure_Impl_MethodCod Index ridx midx (snd x))));
-        [ | rewrite eq_x in H0;  eapply H0 ].
-      intros v Comp_v; simpl in *; inversion_by computes_to_inv; subst.
-      destruct x; simpl @fst in *; simpl @snd in *.
-      unfold ridx' in *.
-      revert H1.
-      Local Transparent CallBagMethod.
-      eapply refine_Mapped_Methods.
-  Qed.
-
-  (*Fixpoint Build_IndexedQueryStructure_Impl_ConstructorDom
-           {indices}
-           {struct indices}
-  : forall (Index : ilist (fun ns : NamedSchema => SearchUpdateTerms (schemaHeading (relSchema ns))) indices)
-             ridx
-             (midx : ConstructorIndex
-                       (BagSig (@Tuple (schemaHeading
-                            (relSchema
-                               (@nth_Bounded NamedSchema string relName
-                                             indices (map_IndexedQS_idx Index ridx ) ))))
-                               (BagSearchTermType
-                                  (ith_Bounded relName Index (map_IndexedQS_idx Index ridx)))
-                               (BagUpdateTermType
-                                  (ith_Bounded relName Index (map_IndexedQS_idx Index ridx))))),
-      (ConstructorDom
-             (BagSig Tuple
-                     (BagSearchTermType
-                        (ith_Bounded relName Index (map_IndexedQS_idx Index ridx)))
-                     (BagUpdateTermType
-                        (ith_Bounded relName Index (map_IndexedQS_idx Index ridx))))
-             midx) -> 
-      (ConstructorDom
-             (namedADTSig
-                (nth_Bounded ADTSigname (Build_IndexedQueryStructure_Impl_Sigs Index)
-                             ridx))
-             (Build_IndexedQueryStructure_Impl_midx ConstructorIndex Index ridx midx)) := 
-    match indices return
-          forall (Index : ilist
-                            (fun ns : NamedSchema =>
-                               SearchUpdateTerms (schemaHeading (relSchema ns)))
-                            indices)
-                 (ridx : BoundedIndex
-                           (map ADTSigname (Build_IndexedQueryStructure_Impl_Sigs Index)))
-                 (midx : ConstructorIndex
-                       (BagSig (@Tuple (schemaHeading
-                            (relSchema
-                               (@nth_Bounded NamedSchema string relName
-                                             indices (map_IndexedQS_idx Index ridx ) ))))
-                               (BagSearchTermType
-                                  (ith_Bounded relName Index (map_IndexedQS_idx Index ridx)))
-                               (BagUpdateTermType
-                                  (ith_Bounded relName Index (map_IndexedQS_idx Index ridx))))),
-            (ConstructorDom
-                   (BagSig Tuple
-                           (BagSearchTermType
-                              (ith_Bounded relName Index (map_IndexedQS_idx Index ridx)))
-                     (BagUpdateTermType
-                        (ith_Bounded relName Index (map_IndexedQS_idx Index ridx))))
-                   midx) -> 
-            (ConstructorDom
-                   (namedADTSig
-                      (nth_Bounded ADTSigname (Build_IndexedQueryStructure_Impl_Sigs Index)
-                                   ridx))
-                   (Build_IndexedQueryStructure_Impl_midx ConstructorIndex Index ridx midx))
-    with
-      | nil => fun _ ridx => BoundedIndex_nil _ ridx
-      | ns :: indices' =>
-        fun Index ridx =>  
-          match ridx with
-            | {| bindex := ridx;
-                 indexb := {|ibound := n;
-                             boundi := nth_n |}|} => 
-              match n return
-                    forall
-                      (Index' : ilist
-                                  (fun ns : NamedSchema =>
-                                     SearchUpdateTerms (schemaHeading (relSchema ns))) (ns :: indices'))
-                      ridx nth_n,
-                      let idx := {| bindex := ridx;
-                                    indexb := {|ibound := n;
-                                                boundi := nth_n |}|} in 
-                      forall (midx : ConstructorIndex (BagSig (@Tuple (schemaHeading
-                                                     (relSchema
-                                                        (@nth_Bounded NamedSchema string relName
-                                                                      (ns :: indices') (map_IndexedQS_idx Index' idx ) ))))
-                                          (BagSearchTermType
-                                             (ith_Bounded relName Index' (map_IndexedQS_idx Index' idx)))
-                                          (BagUpdateTermType
-                                             (ith_Bounded relName Index' (map_IndexedQS_idx Index' idx))))),
-                      (ConstructorDom
-                             (BagSig Tuple
-                                     (BagSearchTermType
-                                        (ith_Bounded relName Index' (map_IndexedQS_idx Index' idx)))
-                                     (BagUpdateTermType
-                                        (ith_Bounded relName Index' (map_IndexedQS_idx Index' idx))))
-                             midx) -> 
-                      (ConstructorDom
-                             (namedADTSig
-                                (nth_Bounded ADTSigname (Build_IndexedQueryStructure_Impl_Sigs Index')
-                                             idx))
-                             (Build_IndexedQueryStructure_Impl_midx ConstructorIndex Index' idx midx))
-              with
-                | 0 => fun Index idx nth_n midx d => d
-                | S n' => fun Index idx nth_n midx d =>
-                            (@Build_IndexedQueryStructure_Impl_ConstructorDom
-                               indices' (ilist_tl Index)
-                               {| bindex := idx;
-                                  indexb := {|ibound := n';
-                                              boundi := nth_n |}|}
-                               midx d)
-              end Index ridx nth_n 
-                            end
-         end.
-
-  Lemma ith_Build_IndexedQueryStructure_Impl_Constructors
-        {indices}
-  : forall
-      (Index : ilist (fun ns : NamedSchema => SearchUpdateTerms (schemaHeading (relSchema ns))) indices )
-      (idx : BoundedIndex
-               (map ADTSigname
-                    (Build_IndexedQueryStructure_Impl_Sigs Index))),
-      Constructors (ith_Bounded ADTSigname (Build_IndexedQueryStructure_Impl_Specs Index) idx) = 
-      eq_rect _ (fun r => forall idx, constructorType (Rep r) _ )
-              (Constructors (eq_rect _ ADT
-                                (@BagSpec (@Tuple (schemaHeading (relSchema (@nth_Bounded NamedSchema string relName
-                                                                                          indices (map_IndexedQS_idx Index idx)))))
-                                          (BagSearchTermType (ith_Bounded _ Index (map_IndexedQS_idx Index idx)))
-                                          (BagUpdateTermType (ith_Bounded _ Index (map_IndexedQS_idx Index idx)))
-                                          (BagMatchSearchTerm (ith_Bounded _ Index (map_IndexedQS_idx Index idx)))
-                                          (BagApplyUpdateTerm (ith_Bounded _ Index (map_IndexedQS_idx Index idx))))
-                                _ (ith_Build_IndexedQueryStructure_Impl_Sigs_eq Index idx)))
-              _ (eq_sym (ith_Build_IndexedQueryStructure_Impl_Specs_eq Index idx)).
-  Proof.
-    destruct idx as [idx [n nth_n]].
-    revert Index idx n nth_n.
-    induction indices; destruct n; simpl; intros; try discriminate; eauto.
-    eapply (IHindices (ilist_tl Index) idx n nth_n).
-  Defined.
-
-  Lemma refine_Mapped_Constructors
-        {indices}
-        (Index : ilist (fun ns : NamedSchema => SearchUpdateTerms (schemaHeading (relSchema ns))) (indices) )
-  :  forall
-      ridx
-      (midx : ConstructorIndex
-                (BagSig Tuple
-                        (BagSearchTermType
-                           (ith_Bounded relName Index (map_IndexedQS_idx Index ridx)))
-                        (BagUpdateTermType
-                           (ith_Bounded relName Index (map_IndexedQS_idx Index ridx)))))
-      d r,
-      Constructors (ith_Bounded ADTSigname (Build_IndexedQueryStructure_Impl_Specs Index) ridx) (Build_IndexedQueryStructure_Impl_midx ConstructorIndex Index ridx midx)
-                   (Build_IndexedQueryStructure_Impl_ConstructorDom Index ridx midx d)
-                   ↝ r ->
-      Constructors
-        (BagSpec (BagMatchSearchTerm (ith_Bounded relName Index (map_IndexedQS_idx Index ridx)))
-                 (BagApplyUpdateTerm (ith_Bounded relName Index (map_IndexedQS_idx Index ridx)))) midx d
-   ↝ map_IndexedQS_Rep' Index ridx r.
-  Proof.
-    intros; pose proof (ith_Build_IndexedQueryStructure_Impl_Constructors Index ridx) as H';
-      simpl ith_Bounded in *; rewrite H' in H; revert H.
-    clear H'.
-    revert d r.
-    eapply Iterate_Dep_Type_BoundedIndex_equiv_1 with (idx := midx).
-    simpl; intuition.
-    simpl in *.
-    revert midx d r H.
-    destruct ridx as [idx [n nth_n]];
-      revert idx n nth_n;
-      unfold IndexedQueryStructure, GetIndexedRelation in *;
-      unfold list_ind, list_rect in *;
-      induction indices; destruct n; simpl; try (intros; discriminate); eauto;
-      eapply IHindices.
-  Qed.
-
-  Check refine_BagImplMethods.
-  Check CallBagImplConstructor.
-    
-  Lemma refine_BagImplConstructors
-        {qs_schema : QueryStructureSchema}
-        (Index : ilist (fun ns : NamedSchema => SearchUpdateTerms (schemaHeading (relSchema ns))) (qschemaSchemas qs_schema) )
-        (DelegateImpls : ilist (fun ns => cADT (namedADTSig ns))
-                               (Build_IndexedQueryStructure_Impl_Sigs Index))
-        (ValidImpl : forall
-                        idx : BoundedIndex
-                                (map ADTSigname
-                                   (Build_IndexedQueryStructure_Impl_Sigs
-                                      Index)),
-                      refineADT
-                        (ith_Bounded ADTSigname
-                           (Build_IndexedQueryStructure_Impl_Specs Index)
-                           idx)
-                        (LiftcADT (ith_Bounded ADTSigname DelegateImpls idx)))
-  :  forall (ridx : BoundedIndex
-                   (map ADTSigname
-                      (Build_IndexedQueryStructure_Impl_Sigs Index)))
-            (midx : ConstructorIndex
-                     (BagSig Tuple
-                             (BagSearchTermType
-                                (ith_Bounded relName Index (map_IndexedQS_idx Index ridx)))
-                             (BagUpdateTermType
-                                (ith_Bounded relName Index (map_IndexedQS_idx Index ridx)))))
-            d,
-       let midx' := Build_IndexedQueryStructure_Impl_midx ConstructorIndex Index ridx midx in
-       let d' := Build_IndexedQueryStructure_Impl_ConstructorDom Index ridx midx d in
-       exists r_o',
-         AbsR (ValidImpl ridx) r_o' (CallBagImplConstructor _ DelegateImpls ridx midx' d')
-         /\ refine (CallBagConstructor _ _ (map_IndexedQS_idx Index ridx) midx d)
-                   (ret (map_IndexedQS_Rep' _ _ r_o')) .
-  Proof.
-    intros.
-    pose proof (ADTRefinementPreservesConstructors (ValidImpl ridx) midx'
-                                                   d' (ReturnComputes _)).
-    inversion_by computes_to_inv; subst.
-    exists x;
-      unfold CallBagImplConstructor; simpl in *; split; simpl.
-    - eassumption.
-    - intros v Comp_v; simpl in *; inversion_by computes_to_inv; subst.
-      Local Transparent CallBagConstructor.
-      eapply refine_Mapped_Constructors; eauto.
-  Qed.
- *)
-
-  Definition Build_IndexedQueryStructure_Impl_AbsR'
-             {qs_schema : QueryStructureSchema}
-             (Index : ilist (fun ns : NamedSchema => SearchUpdateTerms (schemaHeading (relSchema ns))) (qschemaSchemas qs_schema) )
-             (DelegateImpls : ilist (fun ns => cADT (namedADTSig ns))
-                                     (Build_IndexedQueryStructure_Impl_Sigs Index))
-             (ValidImpl :
-                forall idx,
-                  refineADT (ith_Bounded ADTSigname
-                                         (Build_IndexedQueryStructure_Impl_Specs Index) idx)
-                            (LiftcADT (ith_Bounded ADTSigname DelegateImpls idx)))
-             (r_o : IndexedQueryStructure qs_schema Index)
-             (r_n : Build_IndexedQueryStructure_Impl_cRep Index DelegateImpls)
-  : Prop := 
-      @Build_IndexedQueryStructure_Impl_AbsR''
-        qs_schema Index DelegateImpls
-        (fun idx => ValidImpl (map_IndexedQS_idx' Index idx))
-        r_o
-        r_n.
-  
   FullySharpenEachMethod
     (Build_IndexedQueryStructure_Impl_Sigs Index)
     (Build_IndexedQueryStructure_Impl_Specs Index)
@@ -1607,38 +211,138 @@ Methods
   Focus 3.
 
   intros.
-  Opaque CallBagMethod.
+
   simplify with monad laws.
   simpl in *. unfold Build_IndexedQueryStructure_Impl_AbsR' in *.
   match goal with
       H : Build_IndexedQueryStructure_Impl_AbsR'' (qs_schema := ?qs_schema) ?ValidImpl ?r_o ?r_n
       |- context[CallBagMethod (BagIndexKeys := ?Index') ?ridx ?midx ?r_o ?d] =>
       let r_o' := fresh "r_o'" in
-      let AbsR_r_o' := fresh "AbsR_r_o'" in 
-      let refines_r_o := fresh "refines_r_o'" in 
-      destruct (@refine_BagImplMethods qs_schema Index' _ ValidImpl r_o r_n ridx midx d H) as [r_o' [AbsR_r_o' refines_r_o']]; 
+      let AbsR_r_o' := fresh "AbsR_r_o'" in
+      let refines_r_o := fresh "refines_r_o'" in
+      destruct (@refine_BagImplMethods' qs_schema Index' _ ValidImpl r_o r_n ridx H midx d) as [r_o' [refines_r_o' AbsR_r_o']];
+        unfold map_IndexedQS_idx' in refines_r_o', AbsR_r_o'; simpl in refines_r_o', AbsR_r_o';
+        setoid_rewrite refines_r_o'; simpl in *; simplify with monad laws; simpl
+  end.
+
+  match goal with
+    |  [ H : Build_IndexedQueryStructure_Impl_AbsR'' (qs_schema := ?qs_schema)
+                                                     (DelegateImpls := ?DelegateImpl)
+                                                     (fun idx => ?ValidImpl (map_IndexedQS_idx' ?Index idx)) ?r_o ?r_n,
+         H' : AbsR (?ValidImpl ?idx) ?r_o' ?r_n'
+         |- context[
+                { r_n' | Build_IndexedQueryStructure_Impl_AbsR'' (fun idx => ?ValidImpl (map_IndexedQS_idx' ?Index idx))
+                                                        (UpdateIndexedRelation ?r_o ?idx ?r_o') r_n' }
+              ]] => pose proof (refine_pick_val _ (@Update_Build_IndexedQueryStructure_Impl_AbsR'' qs_schema Index DelegateImpl _ r_o r_n idx r_o' r_n' H H'))
+  end.
+  unfold Build_IndexedQueryStructure_Impl_cRep, Build_IndexedQueryStructure_Impl_Sigs, Index
+    in *; simpl in *; setoid_rewrite H0.
+
+  simplify with monad laws.
+
+    Ltac higher_order_2_reflexivity'' :=
+    let x := match goal with |- ?R (ret ?x) (ret (?f ?a ?b)) => constr:(x) end in
+    let f := match goal with |- ?R (ret ?x) (ret (?f ?a ?b)) => constr:(f) end in
+    let a := match goal with |- ?R (ret ?x) (ret (?f ?a ?b)) => constr:(a) end in
+    let b := match goal with |- ?R (ret ?x) (ret (?f ?a ?b)) => constr:(b) end in
+    let x' := (eval pattern a, b in x) in
+    let f' := match x' with ?f' _ _ => constr:(f') end in
+    unify f f';
+      cbv beta;
+      solve [apply reflexivity].
+
+
+  higher_order_2_reflexivity''.
+
+  Focus 3.
+  split.
+  intros.
+  simplify with monad laws.
+  simpl in *; unfold Build_IndexedQueryStructure_Impl_AbsR' in *.
+
+  match goal with
+      H : Build_IndexedQueryStructure_Impl_AbsR'' (qs_schema := ?qs_schema) ?ValidImpl ?r_o ?r_n
+      |- context[CallBagMethod (BagIndexKeys := ?Index') ?ridx ?midx ?r_o ?d] =>
+      let r_o' := fresh "r_o'" in
+      let AbsR_r_o' := fresh "AbsR_r_o'" in
+      let refines_r_o := fresh "refines_r_o'" in
+      destruct (@refine_BagImplMethods' qs_schema Index' _ ValidImpl r_o r_n ridx H midx d) as [r_o' [refines_r_o' AbsR_r_o']];
+        unfold map_IndexedQS_idx' in refines_r_o', AbsR_r_o'; simpl in refines_r_o', AbsR_r_o';
+        setoid_rewrite refines_r_o'; simpl in *; simplify with monad laws; simpl
+  end.
+
+  match goal with
+    |  [ H : Build_IndexedQueryStructure_Impl_AbsR'' (qs_schema := ?qs_schema)
+                                                     (DelegateImpls := ?DelegateImpl)
+                                                     (fun idx => ?ValidImpl (map_IndexedQS_idx' ?Index idx)) ?r_o ?r_n
+         |- context[
+                { r_n' | Build_IndexedQueryStructure_Impl_AbsR'' (fun idx => ?ValidImpl (map_IndexedQS_idx' ?Index idx)) ?r_o r_n'}
+              ]] => setoid_rewrite (refine_pick_val _ H); simplify with monad laws
+  end.
+
+  higher_order_2_reflexivity''.
+
+  split.
+
+  intros.
+  simplify with monad laws.
+  simpl in *; unfold Build_IndexedQueryStructure_Impl_AbsR' in *.
+
+  match goal with
+      H : Build_IndexedQueryStructure_Impl_AbsR'' (qs_schema := ?qs_schema) ?ValidImpl ?r_o ?r_n
+      |- context[CallBagMethod (BagIndexKeys := ?Index') ?ridx ?midx ?r_o ?d] =>
+      let r_o' := fresh "r_o'" in
+      let AbsR_r_o' := fresh "AbsR_r_o'" in
+      let refines_r_o := fresh "refines_r_o'" in
+      destruct (@refine_BagImplMethods' qs_schema Index' _ ValidImpl r_o r_n ridx H midx d) as [r_o' [refines_r_o' AbsR_r_o']];
+        unfold map_IndexedQS_idx' in refines_r_o', AbsR_r_o'; simpl in refines_r_o', AbsR_r_o';
+        setoid_rewrite refines_r_o'; simpl in *; simplify with monad laws; simpl
+  end.
+
+
+
+  match goal with
+      H : Build_IndexedQueryStructure_Impl_AbsR'' (qs_schema := ?qs_schema) ?ValidImpl ?r_o ?r_n
+      |- context[CallBagMethod (BagIndexKeys := ?Index') ?ridx ?midx ?r_o ?d] =>
+      let r_o' := fresh "r_o'" in
+      let AbsR_r_o' := fresh "AbsR_r_o'" in
+      let refines_r_o := fresh "refines_r_o'" in
+      destruct (@refine_BagImplMethods qs_schema Index' _ ValidImpl r_o r_n ridx midx d H) as [r_o' [AbsR_r_o' refines_r_o']];
       unfold map_IndexedQS_idx' in refines_r_o', AbsR_r_o'; simpl in refines_r_o', AbsR_r_o';
       setoid_rewrite refines_r_o'; simpl in *; simplify with monad laws; simpl
   end.
 
+
+
+  match goal with
+      H : Build_IndexedQueryStructure_Impl_AbsR'' (qs_schema := ?qs_schema) ?ValidImpl ?r_o ?r_n
+      |- appcontext[CallBagMethod (BagIndexKeys := ?Index') ?ridx ?midx ?r_o] =>
+      let r_o' := fresh "r_o'" in
+      let AbsR_r_o' := fresh "AbsR_r_o'" in
+      let refines_r_o := fresh "refines_r_o'" in
+      pose (@refine_BagImplMethods qs_schema Index' _ ValidImpl r_o r_n ridx midx d) as [r_o' [AbsR_r_o' refines_r_o']];
+      unfold map_IndexedQS_idx' in refines_r_o', AbsR_r_o'; simpl in refines_r_o', AbsR_r_o';
+      setoid_rewrite refines_r_o'; simpl in *; simplify with monad laws; simpl
+  end.
+
+  match goal with
+    |  [ H : Build_IndexedQueryStructure_Impl_AbsR'' (qs_schema := ?qs_schema)
+                                                     (DelegateImpls := ?DelegateImpl)
+                                                     (fun idx => ?ValidImpl (map_IndexedQS_idx' ?Index idx)) ?r_o ?r_n
+         |- context[
+                { r_n' | Build_IndexedQueryStructure_Impl_AbsR'' (fun idx => ?ValidImpl (map_IndexedQS_idx' ?Index idx)) ?r_o r_n'}
+              ]] => setoid_rewrite (refine_pick_val _ H); simplify with monad laws
+  end.
+
+  Check refine_pick_val.
+
   refine pick val _.
 
-  Focus 2.
-  unfold Build_IndexedQueryStructure_Impl_AbsR''.
-  
-  
-  
-  simpl.
-  Set Printing Implicit.
-  idtac.
-  rewrite H2.
-  
-  pose (e q i _ r i0 b b0 b1 p).
+  apply (@Update_Build_IndexedQueryStructure_Impl_AbsR'' _ _ _ _ _ _ _ _ _ H AbsR_r_o').
 
 
-  
   Focus 3.
-  
+
     [BagSig Book (BuildSearchTermFromAttributes BookSearchTerm);
                            BagSig Order (BuildSearchTermFromAttributes OrderSearchTerm)]
                          (icons _ (BagSpec (SearchTermFromAttributesMatcher BookSearchTerm))
