src/QueryStructure/Automation/AutoDB.v
@@ -12,7 +12,11 @@ Require Export Coq.Bool.Bool Coq.Strings.String
         ADTSynthesis.QueryStructure.Implementation.DataStructures.BagADT.BagADT
         ADTSynthesis.QueryStructure.Implementation.DataStructures.BagADT.BagImplementation
         ADTSynthesis.QueryStructure.Implementation.ListImplementation
-        ADTSynthesis.QueryStructure.Specification.Constraints.tupleAgree.
+        ADTSynthesis.QueryStructure.Specification.Constraints.tupleAgree
+        ADTSynthesis.QueryStructure.Implementation.DataStructures.BagADT.IndexSearchTerms
+        ADTSynthesis.QueryStructure.Implementation.Operations.BagADT.Refinements
+        ADTSynthesis.QueryStructure.Implementation.DataStructures.BagADT.QueryStructureImplementation.
+
 Require Export ADTSynthesis.QueryStructure.Implementation.Operations.
 
 Global Opaque binsert benumerate bfind bcount.
@@ -45,134 +49,667 @@ Ltac lmap A f seq :=
       end
   in aux seq.
 
-(*Ltac makeIndex sc table columns :=
-  set (heading := GetHeading sc table);
-  mkIndex heading ltac:(lmap (Attributes heading)%type ltac:(fun x => constr:(heading/x)) columns).
+  Require Import ADTNotation.BuildComputationalADT.
+  Require Import ADT.ComputationalADT.
 
+  Ltac FullySharpenEachMethod delegateSigs delegateSpecs cRep' cAbsR' :=
+    match goal with
+      |- Sharpened (@BuildADT ?Rep ?consSigs ?methSigs ?consDefs ?methDefs) =>
+      ilist_of_evar
+        (ilist (fun nadt => ComputationalADT.cADT (namedADTSig nadt)) delegateSigs)
+        (fun DelegateImpl Sig => ComputationalADT.cMethodType (cRep' DelegateImpl) (methDom Sig) (methCod Sig))
+        methSigs
+        ltac:(fun cMeths =>
+                ilist_of_evar
+                  (ilist (fun nadt => ComputationalADT.cADT (namedADTSig nadt)) delegateSigs)
+                  (fun DelegateImpl Sig => ComputationalADT.cConstructorType (cRep' DelegateImpl) (consDom Sig))
+                  consSigs
+                  ltac:(fun cCons =>
+                          eapply
+                            (@Notation_Friendly_SharpenFully
+                               _
+                               consSigs
+                               methSigs
+                               consDefs
+                               methDefs
+                               delegateSigs
+                               cRep'
+                               cCons
+                               cMeths
+                               delegateSpecs
+                               cAbsR')));
+        unfold Dep_Type_BoundedIndex_app_comm_cons
+    end; simpl; split.
 
-(** * Tactics galore! *)
+  Fixpoint Build_IndexedQueryStructure_Impl_Sigs
+    {indices : list NamedSchema}
+      (Index : ilist (fun ns : NamedSchema => SearchUpdateTerms (schemaHeading (relSchema ns))) indices)
+    : list NamedADTSig :=
+    match indices as indices return ilist _ indices -> list NamedADTSig with
+      | nil => fun _ => nil
+      | cons ns indices' =>
+        fun Index =>
+          {| ADTSigname := relName ns;
+             namedADTSig :=
+               BagSig (@Tuple (schemaHeading (relSchema ns))) (BagSearchTermType (ilist_hd Index)) (BagUpdateTermType (ilist_hd Index)) |}
+                       :: @Build_IndexedQueryStructure_Impl_Sigs indices' (ilist_tl Index)
+    end Index.
 
-Ltac evarForType T k :=
-  match T with
-  | (?A * ?B)%type =>
-    evarForType A ltac:(fun Av =>
-                          evarForType B ltac:(fun Bv => k (Av, Bv)))
-  | _ => let x := fresh in evar (x : T); let y := eval unfold x in x in clear x; k y
-  end.
+  Fixpoint Build_IndexedQueryStructure_Impl_Specs
+           {indices : list NamedSchema}
+           (Index : ilist (fun ns : NamedSchema => SearchUpdateTerms (schemaHeading (relSchema ns))) indices)
+  : ilist (fun ns => ADT (namedADTSig ns)) (@Build_IndexedQueryStructure_Impl_Sigs indices Index) :=
+    match indices as indices return
+          forall (Index : ilist _ indices),
+            ilist (fun ns : NamedADTSig => ADT (namedADTSig ns))
+                  (@Build_IndexedQueryStructure_Impl_Sigs indices Index)
+    with
+      | nil => fun _ => inil _
+      | cons ns indices' =>
+        fun Index => icons {| ADTSigname := relName ns;
+                              namedADTSig := _ |}
+                           (@BagSpec (@Tuple (schemaHeading (relSchema ns)))
+                                     (BagSearchTermType (ilist_hd Index))
+                                     (BagUpdateTermType (ilist_hd Index))
+                                     (BagMatchSearchTerm (ilist_hd Index))
+                                     (BagApplyUpdateTerm (ilist_hd Index)))
+                           (@Build_IndexedQueryStructure_Impl_Specs indices' (ilist_tl Index))
+    end Index.
 
-Ltac startMethod AbsR :=
-  unfold AbsR in *; split_and; simplify with monad laws.
+  Definition Build_IndexedQueryStructure_Impl_cRep
+           {indices : list NamedSchema}
+           (Index : ilist (fun ns : NamedSchema => SearchUpdateTerms (schemaHeading (relSchema ns))) indices)
+           (DelegateImpls : ilist (fun ns => cADT (namedADTSig ns)) (@Build_IndexedQueryStructure_Impl_Sigs indices Index))
+  : Type
+    :=
+    i2list
+      (fun (ns : NamedADTSig)
+           (index : cADT (namedADTSig ns)) => cRep index) DelegateImpls.
 
-Ltac finishMethod := subst_body; higher_order_1_reflexivity.
+  Fixpoint map_IndexedQS_idx_boundi
+        {indices}
+  : forall
+      n
+      (Index : ilist
+                 (fun ns : NamedSchema =>
+                    SearchUpdateTerms (schemaHeading (relSchema ns)))
+                 indices)
+      idx,
+      nth_error
+        (map ADTSigname (Build_IndexedQueryStructure_Impl_Sigs Index))
+        n = Some idx
+      ->  nth_error (map relName indices) n = Some idx.
+  Proof.
+    refine (match indices with
+              | nil => _
+              | ns :: indices' =>
+                fun n =>
+                  match n return
+                        forall
+                          (Index : ilist
+                                     (fun ns : NamedSchema =>
+                                        SearchUpdateTerms (schemaHeading (relSchema ns)))
+                                     (ns :: indices'))
+                          idx,
+                          nth_error (map ADTSigname (Build_IndexedQueryStructure_Impl_Sigs Index)) n =
+                          Some idx ->
+                          nth_error (map relName (ns :: indices')) n = Some idx
+                  with
+                    | 0 => fun Index idx nth_n => nth_n
+                    | S n' => fun Index => (map_IndexedQS_idx_boundi indices' n' (ilist_tl Index))
+                  end
+            end);
+    simpl; intros; try discriminate; eauto.
+  Defined.
 
-(* These tactics implement initializing the empty database. *)
-Hint Extern 1 (_ ≃ _) => eapply bemptyPlus_correct_DB : StartOfMethod.
+  Definition map_IndexedQS_idx
+             indices
+             (Index : ilist (fun ns : NamedSchema => SearchUpdateTerms (schemaHeading (relSchema ns))) indices )
+             (idx : BoundedIndex
+                      (map ADTSigname
+                           (Build_IndexedQueryStructure_Impl_Sigs Index)))
+  : BoundedIndex (map relName indices) :=
+    {| bindex := bindex idx;
+       indexb := {| ibound := ibound (indexb idx);
+                    boundi := map_IndexedQS_idx_boundi _ Index (boundi (indexb idx))|} |}.
 
-Ltac splitPick :=
-  match goal with
-  | [ |- refine (@Pick ?T _) _ ] => evarForType T ltac:(fun Tv =>
-      rewrite (refine_pick_val' Tv) by (unfold fst, snd; intuition auto with StartOfMethod))
-  end.
+  Fixpoint map_IndexedQS_idx_boundi'
+        {indices}
+  : forall
+      n
+      (Index : ilist
+                 (fun ns : NamedSchema =>
+                    SearchUpdateTerms (schemaHeading (relSchema ns)))
+                 indices)
+      idx,
+      nth_error (map relName indices) n = Some idx
+      -> nth_error
+        (map ADTSigname (Build_IndexedQueryStructure_Impl_Sigs Index))
+        n = Some idx.
+  Proof.
+    refine (match indices with
+              | nil => _
+              | ns :: indices' =>
+                fun n =>
+                  match n return
+                        forall
+                          (Index : ilist
+                                     (fun ns : NamedSchema =>
+                                        SearchUpdateTerms (schemaHeading (relSchema ns)))
+                                     (ns :: indices'))
+                          idx,
+                          nth_error (map relName (ns :: indices')) n = Some idx
+                          -> nth_error (map ADTSigname (Build_IndexedQueryStructure_Impl_Sigs Index)) n = Some idx
+                  with
+                    | 0 => fun Index idx nth_n => nth_n
+                    | S n' => fun Index => (map_IndexedQS_idx_boundi' indices' n' (ilist_tl Index))
+                  end
+            end);
+    simpl; intros; try discriminate; eauto.
+  Defined.
 
-Ltac initializer :=
-  match goal with
-    | [ |- refine (or' <- _; Pick (fun nr' => ?AbsR or' nr')) _ ] =>
-      startMethod AbsR; try splitPick; finishMethod
-  end.
+  Definition map_IndexedQS_idx'
+             indices
+             (Index : ilist (fun ns : NamedSchema => SearchUpdateTerms (schemaHeading (relSchema ns))) indices )
+             (idx : BoundedIndex (map relName indices))
+  : BoundedIndex
+                      (map ADTSigname
+                           (Build_IndexedQueryStructure_Impl_Sigs Index)) :=
+    {| bindex := bindex idx;
+       indexb := {| ibound := ibound (indexb idx);
+                    boundi := map_IndexedQS_idx_boundi' _ Index (boundi (indexb idx))|} |}.
 
-(* We need to avoid bad "simplification" of [bfind_matcher] calls,
- * which hide the right structure for type-class resolution.
- * [simp] defined here is a [simpl] version that prevents such reductions. *)
+  Lemma ith_Build_IndexedQueryStructure_Impl_Sigs_eq
+        {indices}
+  : forall
+      (Index : ilist (fun ns : NamedSchema => SearchUpdateTerms (schemaHeading (relSchema ns))) indices )
+      (idx : BoundedIndex
+               (map ADTSigname
+                    (Build_IndexedQueryStructure_Impl_Sigs Index))),
+      (BagSig (@Tuple (schemaHeading (relSchema ((nth_Bounded relName indices (map_IndexedQS_idx Index idx))))))
+              (BagSearchTermType
+                 (ith_Bounded relName Index (map_IndexedQS_idx Index idx)))
+              (BagUpdateTermType
+                 (ith_Bounded relName Index (map_IndexedQS_idx Index idx))))
+      = namedADTSig
+          (nth_Bounded ADTSigname (Build_IndexedQueryStructure_Impl_Sigs Index) idx).
+  Proof.
+    destruct idx as [idx [n nth_n]].
+    revert Index idx n nth_n.
+    induction indices; destruct n; simpl; intros; try discriminate; eauto.
+    eapply (IHindices (ilist_tl Index) idx n nth_n).
+  Defined.
 
-Ltac hide_bfind_matcher :=
-  repeat match goal with
-         | [ |- appcontext[@bfind_matcher ?a ?b ?c ?d] ] =>
-           remember (@bfind_matcher a b c d)
+  Lemma ith_Build_IndexedQueryStructure_Impl_Specs_eq
+        {indices}
+  : forall
+      (Index : ilist (fun ns : NamedSchema => SearchUpdateTerms (schemaHeading (relSchema ns))) indices )
+      (idx : BoundedIndex
+               (map ADTSigname
+                    (Build_IndexedQueryStructure_Impl_Sigs Index))),
+      ith_Bounded ADTSigname (Build_IndexedQueryStructure_Impl_Specs Index) idx =
+  eq_rect _ ADT
+          (@BagSpec (@Tuple (schemaHeading (relSchema (@nth_Bounded NamedSchema string relName
+                                                                    indices (map_IndexedQS_idx Index idx)))))
+                    (BagSearchTermType (ith_Bounded _ Index (map_IndexedQS_idx Index idx)))
+                    (BagUpdateTermType (ith_Bounded _ Index (map_IndexedQS_idx Index idx)))
+                    (BagMatchSearchTerm (ith_Bounded _ Index (map_IndexedQS_idx Index idx)))
+                    (BagApplyUpdateTerm (ith_Bounded _ Index (map_IndexedQS_idx Index idx))))
+                    _ (ith_Build_IndexedQueryStructure_Impl_Sigs_eq Index idx).
+  Proof.
+    destruct idx as [idx [n nth_n]].
+    revert Index idx n nth_n.
+    induction indices; destruct n; simpl; intros; try discriminate; eauto.
+    eapply (IHindices (ilist_tl Index) idx n nth_n).
+  Defined.
+
+  Definition map_IndexedQS_Rep
+             {indices}
+             (Index : ilist (fun ns : NamedSchema => SearchUpdateTerms (schemaHeading (relSchema ns))) indices )
+             idx
+             (rep : @IndexedEnsemble
+                      (@Tuple
+                         (schemaHeading
+                            (relSchema
+                               (@nth_Bounded NamedSchema string relName
+                                             indices (map_IndexedQS_idx Index idx) )))))
+  : Rep
+      (ith_Bounded ADTSigname
+                   (Build_IndexedQueryStructure_Impl_Specs Index) idx).
+  Proof.
+    destruct idx as [idx [n nth_n]].
+    revert Index idx n nth_n rep.
+    induction indices; destruct n; simpl; intros; try discriminate; eauto.
+    eapply IHindices; eauto.
+  Defined.
+
+  Definition map_IndexedQS_Rep'
+             {indices}
+             (Index : ilist (fun ns : NamedSchema => SearchUpdateTerms (schemaHeading (relSchema ns))) indices )
+             idx
+             (rep : Rep
+                      (ith_Bounded ADTSigname
+                                   (Build_IndexedQueryStructure_Impl_Specs Index)
+                                   (map_IndexedQS_idx' Index idx)))
+  : @IndexedEnsemble
+      (@Tuple
+         (schemaHeading
+            (relSchema
+               (@nth_Bounded NamedSchema string relName
+                             indices idx )))).
+  Proof.
+    destruct idx as [idx [n nth_n]].
+    revert Index idx n nth_n rep.
+    induction indices; destruct n; simpl; intros; try discriminate; eauto.
+    eapply (IHindices (ilist_tl Index)); eauto.
+  Defined.
+
+  Definition Build_IndexedQueryStructure_Impl_AbsR
+             {qs_schema : QueryStructureSchema}
+             (Index : ilist (fun ns : NamedSchema => SearchUpdateTerms (schemaHeading (relSchema ns))) (qschemaSchemas qs_schema) )
+             (DelegateImpls : ilist (fun ns => cADT (namedADTSig ns))
+                                     (Build_IndexedQueryStructure_Impl_Sigs Index))
+             (ValidImpl :
+                forall idx,
+                  refineADT (ith_Bounded ADTSigname
+                                         (Build_IndexedQueryStructure_Impl_Specs Index) idx)
+                            (LiftcADT (ith_Bounded ADTSigname DelegateImpls idx)))
+             (r_o : IndexedQueryStructure qs_schema Index)
+             (r_n : Build_IndexedQueryStructure_Impl_cRep Index DelegateImpls)
+  : Prop :=
+    forall idx,
+      AbsR (ValidImpl idx)
+           (map_IndexedQS_Rep Index idx (GetIndexedRelation r_o (map_IndexedQS_idx Index idx)))
+           (i2th_Bounded ADTSigname r_n idx).
+
+  Definition map_IndexedQS_Rep''
+             {indices}
+             (Index : ilist (fun ns : NamedSchema => SearchUpdateTerms (schemaHeading (relSchema ns))) indices )
+             idx
+             (rep : @IndexedEnsemble
+                      (@Tuple
+                         (schemaHeading
+                            (relSchema
+                               (@nth_Bounded NamedSchema string relName
+                                             indices idx)))))
+  : Rep
+      (ith_Bounded ADTSigname
+                   (Build_IndexedQueryStructure_Impl_Specs Index) (map_IndexedQS_idx' Index idx)).
+  Proof.
+    destruct idx as [idx [n nth_n]].
+    revert Index idx n nth_n rep.
+    induction indices; destruct n; simpl; intros; try discriminate; eauto.
+    eapply IHindices; eauto.
+  Defined.
+
+  Definition Build_IndexedQueryStructure_Impl_AbsR''
+             {qs_schema : QueryStructureSchema}
+             (Index : ilist (fun ns : NamedSchema => SearchUpdateTerms (schemaHeading (relSchema ns))) (qschemaSchemas qs_schema) )
+             (DelegateImpls : ilist (fun ns => cADT (namedADTSig ns))
+                                     (Build_IndexedQueryStructure_Impl_Sigs Index))
+             (ValidImpl :
+                forall idx : BoundedIndex (map relName (qschemaSchemas qs_schema)),
+                  refineADT (ith_Bounded ADTSigname
+                                         (Build_IndexedQueryStructure_Impl_Specs Index) (map_IndexedQS_idx' Index idx))
+                            (LiftcADT (ith_Bounded ADTSigname DelegateImpls (map_IndexedQS_idx' Index idx))))
+             (r_o : IndexedQueryStructure qs_schema Index)
+             (r_n : Build_IndexedQueryStructure_Impl_cRep Index DelegateImpls)
+  : Prop :=
+    forall idx,
+      AbsR (ValidImpl idx)
+           (map_IndexedQS_Rep'' Index idx (GetIndexedRelation r_o idx))
+           (i2th_Bounded ADTSigname r_n (map_IndexedQS_idx' Index idx)).
+
+  Definition CallBagImplMethod
+             {qs_schema : QueryStructureSchema}
+             (Index : ilist (fun ns : NamedSchema => SearchUpdateTerms (schemaHeading (relSchema ns))) (qschemaSchemas qs_schema) )
+             (DelegateImpls : ilist (fun ns => cADT (namedADTSig ns))
+                                    (Build_IndexedQueryStructure_Impl_Sigs Index))
+             idx midx
+             (r_n : Build_IndexedQueryStructure_Impl_cRep Index DelegateImpls) :=
+    cMethods (ith_Bounded ADTSigname DelegateImpls idx) midx (i2th_Bounded _ r_n idx).
+
+  Definition CallBagImplConstructor
+             {qs_schema : QueryStructureSchema}
+             (Index : ilist (fun ns : NamedSchema => SearchUpdateTerms (schemaHeading (relSchema ns))) (qschemaSchemas qs_schema) )
+             (DelegateImpls : ilist (fun ns => cADT (namedADTSig ns))
+                                    (Build_IndexedQueryStructure_Impl_Sigs Index))
+             idx midx :=
+    cConstructors (ith_Bounded ADTSigname DelegateImpls idx) midx .
+
+  Fixpoint Build_IndexedQueryStructure_Impl_midx
+           {indices}
+           (P : ADTSig -> Type)
+  : forall (Index : ilist (fun ns : NamedSchema => SearchUpdateTerms (schemaHeading (relSchema ns))) indices)
+             ridx
+             (midx : P
+                       (BagSig (@Tuple (schemaHeading
+                            (relSchema
+                               (@nth_Bounded NamedSchema string relName
+                                             indices (map_IndexedQS_idx Index ridx ) ))))
+                               (BagSearchTermType
+                                  (ith_Bounded relName Index (map_IndexedQS_idx Index ridx)))
+                               (BagUpdateTermType
+                                  (ith_Bounded relName Index (map_IndexedQS_idx Index ridx))))),
+      P
+        (namedADTSig
+           (nth_Bounded ADTSigname (Build_IndexedQueryStructure_Impl_Sigs Index)
+                        ridx)) :=
+    match indices return
+          forall (Index : ilist
+                            (fun ns : NamedSchema =>
+                               SearchUpdateTerms (schemaHeading (relSchema ns)))
+                            indices)
+                 (ridx : BoundedIndex
+                           (map ADTSigname (Build_IndexedQueryStructure_Impl_Sigs Index)))
+                 (midx : P
+                       (BagSig (@Tuple (schemaHeading
+                            (relSchema
+                               (@nth_Bounded NamedSchema string relName
+                                             indices (map_IndexedQS_idx Index ridx ) ))))
+                               (BagSearchTermType
+                                  (ith_Bounded relName Index (map_IndexedQS_idx Index ridx)))
+                               (BagUpdateTermType
+                                  (ith_Bounded relName Index (map_IndexedQS_idx Index ridx))))),
+      P
+        (namedADTSig
+           (nth_Bounded ADTSigname (Build_IndexedQueryStructure_Impl_Sigs Index)
+                        ridx))
+    with
+      | nil => fun _ ridx => BoundedIndex_nil _ ridx
+      | ns :: indices' =>
+        fun Index ridx =>
+          match ridx with
+            | {| bindex := ridx;
+                 indexb := {|ibound := n;
+                             boundi := nth_n |}|} =>
+              match n return
+                    forall
+                      (Index' : ilist
+                                  (fun ns : NamedSchema =>
+                                     SearchUpdateTerms (schemaHeading (relSchema ns))) (ns :: indices'))
+                      ridx nth_n,
+                      let idx := {| bindex := ridx;
+                                    indexb := {|ibound := n;
+                                                boundi := nth_n |}|} in
+                      P
+                                (BagSig (@Tuple (schemaHeading
+                                                   (relSchema
+                                                      (@nth_Bounded NamedSchema string relName
+                                                                    (ns :: indices') (map_IndexedQS_idx Index' idx ) ))))
+                                        (BagSearchTermType
+                                           (ith_Bounded relName Index' (map_IndexedQS_idx Index' idx)))
+                                        (BagUpdateTermType
+                                           (ith_Bounded relName Index' (map_IndexedQS_idx Index' idx)))) ->
+                      P
+                        (namedADTSig
+                           (nth_Bounded ADTSigname (Build_IndexedQueryStructure_Impl_Sigs Index')
+                                        {| bindex := ridx;
+                                           indexb := {|ibound := n;
+                                                       boundi := nth_n |}|}))
+              with
+                | 0 => fun Index idx nth_n midx => midx
+                | S n' => fun Index idx nth_n midx =>
+                            (@Build_IndexedQueryStructure_Impl_midx
+                               indices' P (ilist_tl Index)
+                               {| bindex := idx;
+                                  indexb := {|ibound := n';
+                                              boundi := nth_n |}|}
+                               midx)
+              end Index ridx nth_n
+                            end
          end.
 
-Ltac reveal_bfind_matcher :=
-  repeat match goal with
-         | [ _ : ?x = @bfind_matcher _ _ _ _ |- _ ] => subst x
-         end.
+  Definition Build_IndexedQueryStructure_Impl_MethodDom
+           {indices}
+  : forall (Index : ilist (fun ns : NamedSchema => SearchUpdateTerms (schemaHeading (relSchema ns))) indices)
+           ridx
+           midx,
+      fst (MethodDomCod
+             (BagSig (@Tuple (schemaHeading (relSchema (nth_Bounded relName indices  ridx))))
+                     (BagSearchTermType
+                        (ith_Bounded relName Index ridx))
+                     (BagUpdateTermType
+                        (ith_Bounded relName Index ridx)))
+             midx)
+    -> fst
+        (MethodDomCod
+           (namedADTSig
+              (nth_Bounded ADTSigname
+                           (Build_IndexedQueryStructure_Impl_Sigs Index) (map_IndexedQS_idx' Index ridx)))
+           (Build_IndexedQueryStructure_Impl_midx MethodIndex Index (map_IndexedQS_idx' Index ridx) midx)).
+  Proof.
+    destruct ridx as [idx [n nth_n]]; revert Index idx n nth_n.
+    induction indices.
+  - destruct n; simpl; discriminate.
+  - destruct n; simpl; eauto.
+    intros; eapply (IHindices (ilist_tl Index) idx n nth_n); eauto.
+  Defined.
 
-Ltac simp := hide_bfind_matcher; simpl; reveal_bfind_matcher.
+  Definition Build_IndexedQueryStructure_Impl_MethodCod
+           {indices}
+  : forall (Index : ilist (fun ns : NamedSchema => SearchUpdateTerms (schemaHeading (relSchema ns))) indices)
+           ridx
+           midx,
+      snd
+        (MethodDomCod
+           (namedADTSig
+              (nth_Bounded ADTSigname
+                           (Build_IndexedQueryStructure_Impl_Sigs Index) (map_IndexedQS_idx' Index ridx)))
+           (Build_IndexedQueryStructure_Impl_midx MethodIndex Index (map_IndexedQS_idx' Index ridx) midx))
+  ->       snd (MethodDomCod
+             (BagSig (@Tuple (schemaHeading (relSchema (nth_Bounded relName indices  ridx))))
+                     (BagSearchTermType
+                        (ith_Bounded relName Index ridx))
+                     (BagUpdateTermType
+                        (ith_Bounded relName Index ridx)))
+             midx)
+.
+  Proof.
+    destruct ridx as [idx [n nth_n]]; revert Index idx n nth_n.
+    induction indices.
+  - destruct n; simpl; discriminate.
+  - destruct n; simpl; eauto.
+    intros; eapply (IHindices (ilist_tl Index) idx n nth_n); eauto.
+  Defined.
 
-Ltac EquivalentBagIsEquivalentIndexedList :=
-  match goal with
-    | [ H: EnsembleBagEquivalence _ ?ens _ |-
-        EnsembleIndexedListEquivalence ?ens _ ] =>
-      solve [apply H]
-  end.
+Lemma ith_Build_IndexedQueryStructure_Impl_Methods
+        {indices}
+  : forall
+      (Index : ilist (fun ns : NamedSchema => SearchUpdateTerms (schemaHeading (relSchema ns))) indices )
+      (idx : BoundedIndex
+               (map ADTSigname
+                    (Build_IndexedQueryStructure_Impl_Sigs Index))),
+      Methods (ith_Bounded ADTSigname (Build_IndexedQueryStructure_Impl_Specs Index) idx) =
+      eq_rect _ (fun r => forall idx, methodType (Rep r) _ _ )
+              (Methods (eq_rect _ ADT
+                                (@BagSpec (@Tuple (schemaHeading (relSchema (@nth_Bounded NamedSchema string relName
+                                                                                          indices (map_IndexedQS_idx Index idx)))))
+                                          (BagSearchTermType (ith_Bounded _ Index (map_IndexedQS_idx Index idx)))
+                                          (BagUpdateTermType (ith_Bounded _ Index (map_IndexedQS_idx Index idx)))
+                                          (BagMatchSearchTerm (ith_Bounded _ Index (map_IndexedQS_idx Index idx)))
+                                          (BagApplyUpdateTerm (ith_Bounded _ Index (map_IndexedQS_idx Index idx))))
+                                _ (ith_Build_IndexedQueryStructure_Impl_Sigs_eq Index idx)))
+              _ (eq_sym (ith_Build_IndexedQueryStructure_Impl_Specs_eq Index idx)).
+  Proof.
+    destruct idx as [idx [n nth_n]].
+    revert Index idx n nth_n.
+    induction indices; destruct n; simpl; intros; try discriminate; eauto.
+    eapply (IHindices (ilist_tl Index) idx n nth_n).
+  Defined.
 
-Ltac concretize1 :=
-  (rewrite refine_List_Query_In by EquivalentBagIsEquivalentIndexedList)
-    || (rewrite refine_Join_List_Query_In by EquivalentBagIsEquivalentIndexedList)
-    || (rewrite refine_List_Query_In_Where; instantiate (1 := _))
-    || rewrite refine_List_For_Query_In_Return_Permutation.
+  Lemma refine_Mapped_Methods
+        {indices}
+        (Index : ilist (fun ns : NamedSchema => SearchUpdateTerms (schemaHeading (relSchema ns))) (indices) )
+  :  forall
+      ridx,
+      forall
+        (r_o : @IndexedEnsemble (@Tuple (schemaHeading (relSchema (nth_Bounded relName indices ridx)))))
+      midx
+      d r s,
+        let ridx' := map_IndexedQS_idx' Index ridx in
+        let midx' := Build_IndexedQueryStructure_Impl_midx MethodIndex Index ridx' midx in
+        let d' := Build_IndexedQueryStructure_Impl_MethodDom Index ridx _ d in
+Methods
+     (ith_Bounded ADTSigname (Build_IndexedQueryStructure_Impl_Specs Index) ridx') midx'
+     (map_IndexedQS_Rep'' Index ridx r_o) d'
+     ↝ (r, s) ->
+Methods
+  (BagSpec (BagMatchSearchTerm (ith_Bounded relName Index ridx))
+           (BagApplyUpdateTerm (ith_Bounded relName Index ridx))) midx r_o d
+   ↝ (map_IndexedQS_Rep' Index ridx r,
+     Build_IndexedQueryStructure_Impl_MethodCod Index ridx midx s).
+  Proof.
+    intros; pose proof (ith_Build_IndexedQueryStructure_Impl_Methods Index ridx') as H';
+    rewrite H' in H; revert H; clear H'.
+    unfold d', midx', ridx' in *; clear ridx' midx' d'.
+    revert r_o d r s.
+    intro; eapply (Iterate_Dep_Type_BoundedIndex_equiv_1) with (idx := midx);
+    simpl.
+    intuition;
+      simpl in *;
+      first [revert midx r_o d r s H
+            | revert midx r_o b a r s H ];
+    try (destruct ridx as [idx [n nth_n]];
+      revert idx n nth_n;
+      unfold IndexedQueryStructure, GetIndexedRelation in *;
+      unfold list_ind, list_rect in *;
+      induction indices; destruct n; simpl; try (intros; discriminate); eauto;
+      eapply IHindices).
+  Qed.
 
-Ltac concretize := repeat concretize1; simpl.
 
-(* Now some tactics that operate while the query is still allowed to vary by permutation. *)
+  Lemma map_indexedqs_Rep'_id
+        {indices}
+  : forall Index idx r_o,
+      map_IndexedQS_Rep'' (indices := indices) Index idx (map_IndexedQS_Rep' Index idx r_o) = r_o.
+  Proof.
+    destruct idx as [idx [n nth_n]]; revert Index idx n nth_n.
+    induction indices; simpl; intros.
+    - destruct n; discriminate.
+    - destruct n; simpl in *; eauto.
+      eapply (IHindices (ilist_tl Index)).
+  Qed.
 
-Ltac equate X Y := let H := fresh in assert (H : X = Y) by reflexivity; clear H.
+  Lemma Update_Build_IndexedQueryStructure_Impl_AbsR''
+        {qs_schema}
+        Index
+  : forall
+      DelegateImpl
+      ValidImpl
+      (r_o : IndexedQueryStructure qs_schema Index)
+      (r_n : Build_IndexedQueryStructure_Impl_cRep Index DelegateImpl)
+      idx r_o' r_n',
+      Build_IndexedQueryStructure_Impl_AbsR'' ValidImpl r_o r_n
+      -> AbsR (ValidImpl idx) r_o' r_n'
+      -> Build_IndexedQueryStructure_Impl_AbsR''
+           ValidImpl
+           (UpdateIndexedRelation r_o idx (map_IndexedQS_Rep' _ _ r_o'))
+           (replace_BoundedIndex2 _ r_n (map_IndexedQS_idx' _ idx) r_n').
+  Proof.
+    intros; intro idx'.
+    destruct (BoundedString_eq_dec idx idx'); subst.
+    - rewrite i2th_replace_BoundIndex_eq, get_update_indexed_eq, map_indexedqs_Rep'_id; eauto.
+    - rewrite i2th_replace_BoundIndex_neq, get_update_indexed_neq; eauto using string_dec.
+      intuition; apply n.
+      destruct idx as [idx [m nth_m]]; destruct idx' as [idx' [n' nth_n']]; simpl in *.
+      injection H1; intros; subst; repeat f_equal.
+      unfold map_IndexedQS_idx' in H1; simpl in H1.
+      apply eq_proofs_unicity_Opt_A; eauto using string_dec.
+  Qed.
 
-Ltac getFst F k :=
-  match type of F with
-  | ?A * ?B -> ?C =>
-    let G := fresh "G" in let p := fresh "p" in let H := fresh "H" in
-    evar (G : A -> C); assert (H : forall p, F p = G (fst p)) by (subst G; intro p;
-      pattern (fst p);
-      match goal with
-      | [ |- (fun t => @?f t = @?g t) _ ] => equate g f; reflexivity
-      end); clear H;
-    let G' := eval unfold G in G in clear G; k G'
-  end.
+  Lemma refine_BagImplMethods'
+        {qs_schema : QueryStructureSchema}
+        (Index : ilist (fun ns : NamedSchema => SearchUpdateTerms (schemaHeading (relSchema ns))) (qschemaSchemas qs_schema) )
+        (DelegateImpls : ilist (fun ns => cADT (namedADTSig ns))
+                               (Build_IndexedQueryStructure_Impl_Sigs Index))
+        ValidImpl
+  :  forall (r_o : IndexedQueryStructure qs_schema Index)
+            (r_n : Build_IndexedQueryStructure_Impl_cRep Index DelegateImpls)
+            ridx,
+       let ridx' := map_IndexedQS_idx' Index ridx in
+       Build_IndexedQueryStructure_Impl_AbsR'' ValidImpl r_o r_n ->
+            forall (midx : MethodIndex
+                     (BagSig Tuple
+                             (BagSearchTermType
+                                (ith_Bounded relName Index (map_IndexedQS_idx Index ridx')))
+                             (BagUpdateTermType
+                                (ith_Bounded relName Index (map_IndexedQS_idx Index ridx')))))
+                   (d : fst
+                          (MethodDomCod
+                             (BagSig (@Tuple (schemaHeading (relSchema (nth_Bounded relName (qschemaSchemas qs_schema) ridx))))
+                                     (BagSearchTermType (ith_Bounded relName Index ridx))
+                                     (BagUpdateTermType (ith_Bounded relName Index ridx))) midx)),
+       let midx' := Build_IndexedQueryStructure_Impl_midx MethodIndex Index ridx' midx in
+       let d' := Build_IndexedQueryStructure_Impl_MethodDom Index ridx _ d in
+       exists r_o',
+                  refine (CallBagMethod ridx midx r_o d)
+                  (ret (map_IndexedQS_Rep' _ _ r_o',
+                        Build_IndexedQueryStructure_Impl_MethodCod Index ridx _
+                                                                   (snd (CallBagImplMethod (map_IndexedQS_idx' Index ridx) midx' r_n d'))))
+                /\ AbsR (ValidImpl ridx) r_o' (fst (CallBagImplMethod ridx' midx' r_n d')).
+    intros.
+    pose proof (ADTRefinementPreservesMethods (ValidImpl ridx) midx'
+                                              (map_IndexedQS_Rep'' Index ridx
+                                                                 (GetIndexedRelation r_o ridx))
+                                              (i2th_Bounded _ r_n ridx') d' (H ridx) (ReturnComputes _)).
+    Local Arguments map_IndexedQS_Rep : simpl never.
+    inversion_by computes_to_inv; subst.
+    exists (fst x);
+      unfold CallBagImplMethod; simpl in *.
+      split; simpl.
+      - pose proof (f_equal snd H3) as eq_x; simpl in eq_x.
+        assert (refine (CallBagMethod ridx midx r_o d)
+                       (ret
+                          (map_IndexedQS_Rep' Index ridx (fst x),
+                           Build_IndexedQueryStructure_Impl_MethodCod Index ridx midx (snd x))));
+          [ | rewrite eq_x in H0;  eapply H0 ].
+        intros v Comp_v; simpl in *; inversion_by computes_to_inv; subst.
+        destruct x; simpl @fst in *; simpl @snd in *.
+        unfold ridx' in *.
+        revert H1.
+        Local Transparent CallBagMethod.
+        eapply refine_Mapped_Methods.
+      - pose proof (f_equal fst H3) as eq_x0; simpl in eq_x0.
+        rewrite eq_x0 in H2; simpl in H2; apply H2.
+  Qed.
 
-Ltac getSnd F k :=
-  match type of F with
-  | ?A * ?B -> ?C =>
-    let G := fresh "G" in let p := fresh "p" in let H := fresh "H" in
-    evar (G : B -> C); assert (H : forall p, F p = G (snd p)) by (subst G; intro p;
-      pattern (snd p);
-      match goal with
-      | [ |- (fun t => @?f t = @?g t) _ ] => equate g f; reflexivity
-      end); clear H;
-    let G' := eval unfold G in G in clear G; k G'
-  end.
+  Opaque CallBagMethod.
 
-Theorem map_ident : forall A ls, map (fun x : A => x) ls = ls.
-Proof.
-  induction ls; simpl; intuition congruence.
-Qed.
 
-Ltac asPerm_indep :=
-  match goal with
-    | _ => setoid_rewrite map_ident
-    | _ => setoid_rewrite map_flat_map; simp
-    | _ => setoid_rewrite map_map; simp
-    | _ => setoid_rewrite (bfind_correct _)
-    | [ |- context[filter ?F _] ] =>
-      getFst F ltac:(fun f => rewrite (filter_join_fst f))
-                      || getSnd F ltac:(fun f => rewrite (filter_join_snd f))
-    | [ |- context[filter _ (Join_Lists ?ls1 (filter ?f ?ls2))] ] =>
-      (* The check below prevent this rule from creating an infinite loop
-         when asPerm_indep is called repeatedly *)
-      match ls1 with (filter _ _) => fail 1 | _ => idtac end;
-      (* If ls1 is not a filter, though, it's probably best to swap the two
-         lists before calling rewrite filter_join_lists, since filter_join
-         _lists produces code that loops on the ls1 first *)
-      setoid_rewrite (swap_joins ls1 (filter f ls2)); trickle_swap; simp
-    | _ => setoid_rewrite filter_join_lists; simp
-    | _ => setoid_rewrite <- filter_and
-  end.
+  Definition Build_IndexedQueryStructure_Impl_AbsR'
+             {qs_schema : QueryStructureSchema}
+             (Index : ilist (fun ns : NamedSchema => SearchUpdateTerms (schemaHeading (relSchema ns))) (qschemaSchemas qs_schema) )
+             (DelegateImpls : ilist (fun ns => cADT (namedADTSig ns))
+                                    (Build_IndexedQueryStructure_Impl_Sigs Index))
+             (ValidImpl :
+                forall idx,
+                  refineADT (ith_Bounded ADTSigname
+                                         (Build_IndexedQueryStructure_Impl_Specs Index) idx)
+                            (LiftcADT (ith_Bounded ADTSigname DelegateImpls idx)))
+             (r_o : IndexedQueryStructure qs_schema Index)
+             (r_n : Build_IndexedQueryStructure_Impl_cRep Index DelegateImpls)
+  : Prop :=
+      @Build_IndexedQueryStructure_Impl_AbsR''
+        qs_schema Index DelegateImpls
+        (fun idx => ValidImpl (map_IndexedQS_idx' Index idx))
+        r_o
+        r_n.
+
+Arguments BuildIndexSearchTerm : simpl never.
+Arguments MatchIndexSearchTerm : simpl never.
+Opaque Initialize_IndexedQueryStructure.
 
 Ltac fields storage :=
   match eval cbv delta [storage] in storage with
   | let src := ?X in _ => X
   end.
 
-Ltac makeEvar T k :=
-  let x := fresh in evar (x : T); let y := eval unfold x in x in clear x; k y.
+  Ltac prove_extensional_eq :=
+  clear;
+  unfold ExtensionalEq;
+  destruct_ifs; first [ solve [intuition] | solve [exfalso; intuition] | idtac ].
+
 
 Ltac findMatchingTerm fds s k :=
   match fds with
@@ -194,7 +731,7 @@ Ltac createTerm f fds tail fs k :=
   end.
 
 (* Get the heading of SC, then *)
-Ltac makeTerm storage fs SC fds tail k :=
+Ltac makeTerm fs SC fds tail k :=
   match eval hnf in SC with
   | Build_Heading ?f =>
     createTerm f fds tail fs k
@@ -203,433 +740,522 @@ Ltac makeTerm storage fs SC fds tail k :=
 (* Given a storage schema [SC], a filter [F], and a
    tactic [k] which processes filters, convert [F] into
    a search term (a list of boolean functions over the tuples in
-   [SC]. *)
+   [SC]). *)
 Ltac findGoodTerm SC F k :=
   match F with
-  | fun a => ?[@?f a] =>
-    match type of f with
-    | forall a, {?X = _!?fd} + {_} => k (fd, X) (@nil (TSearchTermMatcher SC))
-    | forall a, {_!?fd = ?X} + {_} => k (fd, X) (@nil (TSearchTermMatcher SC))
-    | forall a, {?X = _``?fd} + {_} => k (fd, X) (@nil (TSearchTermMatcher SC))
-    | forall a, {_``?fd = ?X} + {_} => k (fd, X) (@nil (TSearchTermMatcher SC))
-    end
-  | fun a => (@?f a) && (@?g a) =>
-    findGoodTerm SC f ltac:(fun fds1 tail1 =>
-      findGoodTerm SC g ltac:(fun fds2 tail2 =>
-        k (fds1, fds2) (tail1 ++ tail2)%list))
-  | _ => k tt (F :: nil)
-  end.
-
-Ltac useIndex storage :=
-  match goal with
-    (* If we've already filtered, don't do it again*)
-    | [ |- context[@filter Tuple (@bfind_matcher _ _ _ _ _ _) _ ] ] => fail 1
-    | [ |- context[@filter Tuple ?F _ ] ] =>
-      let fs := fields storage in
-      match type of fs with
-        | list (Attributes ?SC) =>
-          findGoodTerm SC F ltac:(fun fds tail =>
-            let tail := eval simpl in tail in
-              makeTerm storage fs SC fds tail
-              ltac:(fun tm => rewrite filter over storage using search term tm))
+    | fun a => ?[@?f a] =>
+      match type of f with
+        | forall a, {?X = _!?fd} + {_} => k (fd, X) (fun _ : @Tuple SC => true)
+        | forall a, {_!?fd = ?X} + {_} => k (fd, X) (fun _ : @Tuple SC => true)
+        | forall a, {?X = _``?fd} + {_} => k (fd, X) (fun _ : @Tuple SC => true)
+        | forall a, {_``?fd = ?X} + {_} => k (fd, X) (fun _ : @Tuple SC => true)
       end
+    | fun a => (@?f a) && (@?g a) =>
+      findGoodTerm SC f ltac:(fun fds1 tail1 =>
+                                findGoodTerm SC g ltac:(fun fds2 tail2 =>
+                                                          k (fds1, fds2) (fun tup : @Tuple SC => (tail1 tup) && (tail2 tup))))
+    | _ => k tt F
   end.
 
-Ltac find_usage F k :=
-  match F with
-    | fun x => map ?G (@?F' x) =>
-      let T := type of G in
-      find_usage F' k
-    | fun x => filter ?G (@?F' x) =>
-      let T := type of G in
-      find_usage F' k
-    | fun x => map (fun y => @?G x y) (@?F' x) =>
-      k G
-    | fun x => filter (fun y => @?G x y) (@?F' x) =>
-      k G
+Ltac find_simple_search_term qs_schema idx filter_dec search_term :=
+  match type of search_term with
+    | BuildIndexSearchTerm ?attr =>
+     let SC := constr:(QSGetNRelSchemaHeading qs_schema idx) in
+              findGoodTerm SC filter_dec
+                           ltac:(fun fds tail =>
+                                   let tail := eval simpl in tail in
+                                       makeTerm attr SC fds tail
+                                                ltac:(fun tm => pose tm; try unify tm search_term;
+                                                      unfold ExtensionalEq, MatchIndexSearchTerm;
+                                                      simpl; intro; try prove_extensional_eq))
   end.
 
-Ltac findGoodTerm_dep SC F k :=
+Ltac implement_QSDeletedTuples find_search_term :=
+match goal with
+    [ H : @DelegateToBag_AbsR ?qs_schema ?indices ?r_o ?r_n
+      |- context[Pick (QSDeletedTuples ?r_o ?idx ?DeletedTuples)] ] =>
+    let filter_dec := eval simpl in (@DecideableEnsembles.dec _ DeletedTuples _) in
+    let idx_search_update_term := eval simpl in (ith_Bounded relName indices idx) in
+    let search_term_type := eval simpl in (BagSearchTermType idx_search_update_term) in
+    let search_term_matcher := eval simpl in (BagMatchSearchTerm idx_search_update_term) in
+        makeEvar search_term_type
+                 ltac: (fun search_term =>
+          let eqv := fresh in
+          assert (ExtensionalEq filter_dec (search_term_matcher search_term)) as eqv;
+            [ find_search_term qs_schema idx filter_dec search_term
+            | let H' := fresh in
+              pose (@refine_BagADT_QSDelete_fst _ _ r_o r_n H idx DeletedTuples _ search_term) as H';
+                setoid_rewrite (H' eqv); clear H' eqv])
+end.
+
+Ltac implement_EnsembleDelete_AbsR find_search_term :=
+  match goal with
+      [ H : @DelegateToBag_AbsR ?qs_schema ?indices ?r_o ?r_n
+        |- context[{r_n' | DelegateToBag_AbsR
+                             (UpdateUnConstrRelation ?r_o ?idx
+                                                     (EnsembleDelete (GetUnConstrRelation ?r_o ?idx)
+                                                                     ?DeletedTuples)) r_n'}]] =>
+      let filter_dec := eval simpl in (@DecideableEnsembles.dec _ DeletedTuples _) in
+      let idx_search_update_term := eval simpl in (ith_Bounded relName indices idx) in
+      let search_term_type := eval simpl in (BagSearchTermType idx_search_update_term) in
+      let search_term_matcher := eval simpl in (BagMatchSearchTerm idx_search_update_term) in
+          makeEvar search_term_type
+                   ltac:(fun search_term =>
+                           let eqv := fresh in
+                           assert (ExtensionalEq filter_dec (search_term_matcher search_term)) as eqv;
+                         [ find_search_term qs_schema idx filter_dec search_term
+                         | let H' := fresh in
+                           pose (@refine_BagADT_QSDelete_snd _ _ r_o r_n H idx DeletedTuples _ search_term) as H';
+                             setoid_rewrite (H' eqv); clear H' eqv] )
+  end.
+
+Ltac implement_Enumerate_filter find_search_term :=
+  match goal with
+      [ H : @DelegateToBag_AbsR ?qs_schema ?indices ?r_o ?r_n
+        |- context[For (l <- CallBagMethod ?idx {| bindex := "Enumerate"|} ?r_n0 ();
+                        (List_Query_In (filter (@DecideableEnsembles.dec _ ?DeletedTuples _) (snd l))
+                                            ?resultComp))]] =>
+      let filter_dec := eval simpl in (@DecideableEnsembles.dec _ DeletedTuples _) in
+      let idx_search_update_term := eval simpl in (ith_Bounded relName indices idx) in
+      let search_term_type := eval simpl in (BagSearchTermType idx_search_update_term) in
+      let search_term_matcher := eval simpl in (BagMatchSearchTerm idx_search_update_term) in
+          makeEvar search_term_type
+                   ltac:(fun search_term =>
+                           let eqv := fresh in
+                           assert (ExtensionalEq filter_dec (search_term_matcher search_term)) as eqv;
+                         [ find_search_term qs_schema idx filter_dec search_term
+                         | let H' := fresh in
+                           pose (@refine_Query_For_In_Find _ _ string _ _ H idx filter_dec
+                                                           search_term resultComp) as H';
+                         setoid_rewrite (H' eqv); clear H'])
+  end.
+
+Ltac implement_Pick_DelegateToBag_AbsR_observer :=
+  match goal with
+      [H : @DelegateToBag_AbsR ?qs_schema ?indices ?r_o ?r_n
+       |- context[{r_n' : IndexedQueryStructure ?qs_schema ?indices | DelegateToBag_AbsR ?r_o r_n'}] ]
+      => setoid_rewrite (refine_pick_val (@DelegateToBag_AbsR qs_schema indices r_o) H)
+  end.
+
+  Add Parametric Morphism
+      (A : Type)
+      (f : A -> Type)
+      (As : list A)
+      (a : A)
+      (l' : list (ilist f As))
+      : (@Join_Lists A f As a l')
+      with signature
+      (pointwise_relation _ refine) ==> refine
+        as refine_Join_Lists.
+  Proof.
+    unfold pointwise_relation; simpl; intros.
+    induction l'; unfold Join_Lists; simpl.
+    - reflexivity.
+    - rewrite H; setoid_rewrite IHl'; reflexivity.
+  Qed.
+
+Lemma refine_Join_Enumerate_Swap
+      qs_schema BagIndexKeys
+        (ResultT : Type) :
+    forall r_o (r_n : IndexedQueryStructure qs_schema BagIndexKeys),
+      DelegateToBag_AbsR r_o r_n ->
+      forall (idx idx' : BoundedString)
+             (resultComp : _ -> Comp (list ResultT)),
+        refine (l <- CallBagMethod idx {|bindex := "Enumerate" |} r_n ();
+                l' <- (Join_Lists (Build_single_Tuple_list (snd l))
+                                  (fun _ => l <- (CallBagMethod idx' {|bindex := "Enumerate" |} r_n ());
+                                   ret (snd l)));
+                List_Query_In l' resultComp)
+               (l <- CallBagMethod idx' {|bindex := "Enumerate" |} r_n ();
+                l' <- (Join_Lists (Build_single_Tuple_list (snd l))
+                                  (fun _ => l <- (CallBagMethod idx {|bindex := "Enumerate" |} r_n ());
+                                   ret (snd l)));
+                List_Query_In l' (fun tup_pair => (resultComp (icons _ (ilist_hd (ilist_tl tup_pair)) (icons _ (ilist_hd tup_pair) (inil _)))))).
+  Proof.
+  Admitted.
+
+(* implement_In' implements [UnConstrQuery_In] in a variety of contexts. *)
+Ltac implement_In' :=
+  match goal with
+    (* Implement a List_Query_In of a list [l] applied to a UnConstrQuery_In [idx]
+        by enumerating [idx] with a method call and joining the result with [l] *)
+    | [H : @DelegateToBag_AbsR ?qs_schema ?indexes ?r_o ?r_n
+       |- context[fun b' : ?ElementT => List_Query_In (@?l b') (fun b => UnConstrQuery_In (ResultT := ?resultT) ?r_o ?idx (@?f b' b) )] ] =>
+      let H' := eval simpl in
+      (fun (b' : ElementT) => refine_Join_Query_In_Enumerate' H idx (f b') (l b')) in
+          setoid_rewrite H'
+
+    (* Implement a 'naked' UnConstrQuery_In as a call to enumerate *)
+    | [H : @DelegateToBag_AbsR ?qs_schema ?indexes ?r_o ?r_n
+       |- context[UnConstrQuery_In (ResultT := ?resultT) ?r_o ?idx ?f] ] =>
+      let H' := eval simpl in (refine_Query_In_Enumerate H (idx := idx) f) in
+          setoid_rewrite H'
+
+    (* Implement a UnConstrQuery_In under a single binder as a call to enumerate *)
+    | [H : @DelegateToBag_AbsR ?qs_schema ?indexes ?r_o ?r_n
+       |- context[fun b => UnConstrQuery_In (ResultT := ?resultT) ?r_o ?idx (@?f b) ] ] =>
+      let H' := eval simpl in
+      (fun b => @refine_Query_In_Enumerate qs_schema indexes _ r_o r_n H idx (f b)) in
+          setoid_rewrite H'
+  end.
+
+Ltac implement_In :=
+  (* First simplify any large terms [i.e. Rep, BagSpec, snd, and MethodDomCod
+     that might slow down setoid rewriting *)
+  simpl in *;
+  (* The repeatedly implement [In]s *)
+  repeat implement_In'.
+
+
+  Fixpoint Join_ListsT (Ts : list Type) : Type
+    :=
+      match Ts with
+        | [] => unit
+        | [A] => A
+        | A :: Cs => prod A (Join_ListsT Cs)
+      end.
+
+  Lemma ExtensionalEq_andb {A} :
+    forall (f g f' g' : A -> bool),
+      ExtensionalEq f f'
+      -> ExtensionalEq g g'
+      -> ExtensionalEq (fun a => f a && g a) (fun a => f' a && g' a).
+  Proof.
+    unfold ExtensionalEq; intros; congruence.
+  Qed.
+
+  Lemma ExtensionalEq_andb_true {A} :
+    forall (f f' : A -> bool),
+      ExtensionalEq f f'
+      -> ExtensionalEq f (fun a => f' a && (fun _ => true) a).
+  Proof.
+    unfold ExtensionalEq; intros.
+    rewrite andb_true_r; apply H.
+  Qed.
+
+  Ltac split_filters k :=
+    match goal with
+      | |- ExtensionalEq (fun a => (@?f a) && (@?g a)) ?b =>
+        let fT := type of f in
+        let gT := type of g in
+        makeEvar
+          fT
+          ltac:(fun f' =>
+                  makeEvar gT ltac:(fun g' =>
+                                      apply (@ExtensionalEq_andb _ f g f' g');
+                                    [ first [split_filters | k ] | first [split_filters | k]] ))
+      | |- ExtensionalEq (fun a => (@?f a)) ?b =>
+        let fT := type of f in
+        makeEvar
+          fT
+          ltac:(fun f' => k)
+    end.
+
+  (* Convert List_Query_In Where Clauses into a filter using search terms. *)
+  Ltac convert_Where_to_search_term :=
+    (* First replace Where clauses with test functions. *)
+    simpl; repeat (setoid_rewrite refine_List_Query_In_Where;
+                   instantiate (1 := _)); simpl;
+    (* Combine different filters into a single function. *)
+    repeat setoid_rewrite <- filter_and;
+    (* Now break the functions up again and find search term replacements for each. *)
+    match goal with
+        |- context [List_Query_In (filter ?f _) _] =>
+        let T := type of f in
+        makeEvar T
+                 ltac:(fun g =>
+                         let eqv := fresh in
+                         assert (ExtensionalEq f g) as eqv;
+                       [ apply ExtensionalEq_andb_true; split_filters idtac
+                       | setoid_rewrite (filter_by_equiv f g eqv)])
+    end.
+
+  Ltac equate X Y := let H := fresh in assert (H : X = Y) by reflexivity; clear H.
+
+    Definition unit_Heading :=
+      {| Attributes := unit;
+         Domain := fun _ => unit |}.
+
+    Definition unit_Tuple : @Tuple unit_Heading := id.
+
+    Ltac get_ithDefault f n k :=
+      match type of f with
+        | ilist (@Tuple) ?A -> ?C =>
+          let G := fresh "G" in
+          let p := fresh "p" in
+          let H := fresh "H" in
+          let proj := fresh "proj" in
+          let proj := eval simpl in
+          (fun b : ilist (@Tuple) A => ith_default unit_Heading unit_Tuple b n) in
+          evar (G : @Tuple (nth_default unit_Heading A n) -> C);
+             assert (H : forall p,
+                          f p = G (proj p)) by
+              (subst G; intro p;
+               let p' := eval simpl in (proj p) in
+                   pattern p';
+               match goal with
+                 | [ |- (fun t => @?f t = @?g t) _ ] => equate g f; reflexivity
+               end); clear H;
+        let G' := eval unfold G in G in clear G; k G'
+      end.
+
+    Ltac get_ithDefault_pair f m n k :=
+      match type of f with
+        | ilist (@Tuple) ?A -> ?C =>
+          let G := fresh "G" in
+          let p := fresh "p" in
+          let H := fresh "H" in
+          let proj1 := fresh "proj" in
+          let proj2 := fresh "proj" in
+          let proj1 := eval simpl in
+          (fun b : ilist (@Tuple) A => ith_default unit_Heading unit_Tuple b m) in
+          let proj2 := eval simpl in
+          (fun b : ilist (@Tuple) A => ith_default unit_Heading unit_Tuple b n)
+            in evar (G : @Tuple (nth_default unit_Heading A m)
+                         -> @Tuple (nth_default unit_Heading A n)
+                         -> C);
+             assert (H : forall p,
+                           f p = G (proj1 p) (proj2 p)) by
+              ( subst G; intro p;
+               let p1 := eval simpl in (proj1 p) in
+               let p2 := eval simpl in (proj2 p) in
+               pattern p1, p2;
+                 match goal with
+                   | [ |- (fun t t' => @?f t t' = @?g t t') _ _ ] => equate f g; reflexivity
+                 end); clear H;
+             let G' := eval unfold G in G in clear G; k G'
+      end.
+
+ (* Build pairs of fields + their values. *)
+    Ltac findGoodTerm_dep SC F k :=
   match F with
   | fun (a : ?T) b => ?[@?f a b] =>
     match type of f with
-    | forall a b, {@?X a = _!?fd} + {_} => k (fd, X) (fun _ : T => @nil (TSearchTermMatcher SC))
-    | forall a b, {_!?fd = @?X a} + {_} => k (fd, X) (fun _ : T => @nil (TSearchTermMatcher SC))
-    | forall a b, {@?X a = _``?fd} + {_} => k (fd, X) (fun _ : T => @nil (TSearchTermMatcher SC))
-    | forall a b, {_``?fd = @?X a} + {_} => k (fd, X) (fun _ : T => @nil (TSearchTermMatcher SC))
+    | forall a b, {@?X a = _!?fd} + {_} => k (fd, X) (fun _ : @Tuple SC => true)
+    | forall a b, {_!?fd = @?X a} + {_} => k (fd, X) (fun _ : @Tuple SC => true)
+    | forall a b, {@?X a = _``?fd} + {_} => k (fd, X) (fun _ : @Tuple SC => true)
+    | forall a b, {_``?fd = @?X a} + {_} => k (fd, X) (fun _ : @Tuple SC => true)
     end
   | fun (a : ?T) b => (@?f a b) && (@?g a b) =>
     findGoodTerm_dep SC f ltac:(fun fds1 tail1 =>
       findGoodTerm_dep SC g ltac:(fun fds2 tail2 =>
-        k (fds1, fds2) (fun x : T => tail1 x ++ tail2 x)%list))
-  | _ => k tt (fun x => F x :: nil)
+        k (fds1, fds2) (fun tup : @Tuple SC => (tail1 tup) && (tail2 tup))))
+  | _ => k tt F
   end.
 
-Ltac createTerm_dep dom SC f fds fs k :=
+    (* Build search a search term from the list of attribute + value pairs in fs. *)
+Ltac createTerm_dep dom fs f fds tail k :=
   match fs with
   | nil =>
-    k (fun x : dom => @nil (TSearchTermMatcher SC))
+    k (fun x : dom => tail)
   | ?s :: ?fs' =>
-    createTerm_dep dom SC f fds fs' ltac:(fun rest =>
-      findMatchingTerm fds s ltac:(fun X =>
-        k (fun x : dom => (Some (X x), rest x)))
-      || k (fun x : dom => (@None (f s), rest x)))
+    createTerm_dep dom fs' f fds tail
+      ltac:(fun rest =>
+               findMatchingTerm fds s
+                   ltac:(fun X =>
+                           k (fun x : dom => (Some (X x), rest x)))
+                          || k (fun x : dom => (@None (f s), rest x)))
   end.
 
-Ltac makeTerm_dep SC storage dom fds k :=
-  let fs := fields storage in
+(* Get the heading of [SC] before building the search term. *)
+Ltac makeTerm_dep dom fs SC fds tail k :=
   match eval hnf in SC with
-    | Build_Heading ?f =>
-      createTerm_dep dom SC f fds fs k
+  | Build_Heading ?f =>
+    createTerm_dep dom fs f fds tail k
   end.
 
-Ltac useIndex_dep storage :=
-  let fs := fields storage in
-  match type of fs with
-    | list (Attributes ?SC) =>
-      match goal with
-        | [ |- context[fun x : ?dom => @?F x] ] => find_usage F ltac:(fun G =>
-          findGoodTerm_dep SC G ltac:(fun fds rest =>
-            let rest := eval simpl in rest in
-            makeTerm_dep SC storage dom fds ltac:(fun tm =>
-              let tm := eval simpl in tm in
-                rewrite dependent filter G over storage
-                        using dependent search term tm)))
-      end
+Definition Dep_SearchTerm_Wrapper {A} {heading}
+           (search_term_dep : @Tuple heading -> A)
+           (tup : @Tuple heading) : A := search_term_dep tup.
+
+Ltac find_simple_search_term_dep qs_schema idx dom filter_dec search_term :=
+  match type of search_term with
+    | ?dom -> BuildIndexSearchTerm ?attr =>
+      let SC := constr:(QSGetNRelSchemaHeading qs_schema idx) in
+      findGoodTerm_dep SC filter_dec
+                       ltac:(fun fds tail =>
+                               let tail := eval simpl in tail in
+                                   makeTerm_dep dom attr SC fds tail
+                                                ltac:(fun tm => pose tm;
+                                                      (* unification fails if I don't pose tm first... *)
+                                                      unify (Dep_SearchTerm_Wrapper tm) search_term;
+                                                      unfold ExtensionalEq, MatchIndexSearchTerm;
+                                                      simpl; intros;
+                                                      try prove_extensional_eq))
   end.
 
-Ltac useDeleteIndex :=
-  match goal with
-      [ H : EnsembleBagEquivalence ?bag_plus (@GetUnConstrRelation ?qsSchema ?qs ?Ridx) ?bag
-        |- context[Pick (QSDeletedTuples ?qs ?Ridx ?DeletedTuples)] ] =>
-      let dec := constr:(@dec _ DeletedTuples _) in
-      let storage := bag_plus in
-      let fs := fields storage in
-      match type of fs with
-        | list (Attributes ?SC) =>
-          findGoodTerm SC dec ltac:(fun fds tail =>
-            let tail := eval simpl in tail in
-              makeTerm storage fs SC fds tail
-              ltac:(fun tm =>
-                      rewrite (@bdelete_correct_DB_fst
-                                 qsSchema qs Ridx bag_plus
-                                 bag H DeletedTuples _ tm) by prove_extensional_eq))
-      end
-    end; rewrite refineEquiv_bind_unit; simpl.
+(* Find the name of a schema [schemas] with the same heading as [heading] *)
 
-Ltac asPerm_dep' storage := useIndex storage || useIndex_dep storage.
-Ltac asPerm_dep storages :=
-  asPerm_dep' storages
-          || match storages with
-             | (?s1, ?s2) => asPerm_dep s1 || asPerm_dep s2
-             end.
-
-Ltac asPerm' storages := asPerm_indep || asPerm_dep storages.
-Ltac asPerm storages := repeat (asPerm' storages).
-
-(* A final cleanup phase, applying a few helpful rewrites *)
-
-Ltac cleanup := repeat (setoid_rewrite length_flat_map
-                     || setoid_rewrite map_length
-                     || setoid_rewrite bcount_correct).
-
-(* After doing all the optimizations we want in permutation land, we commit to a list. *)
-
-Lemma refine_count : forall A B C a (f : A -> B) (g : B -> Comp C),
-                       refine (x <- (l <- ret a; ret (f l)); g x) (x <- ret (f a); g x).
-Proof.
-  intros; simplify with monad laws; do 2 intro.
-  apply computes_to_inv in H; firstorder.
-  apply computes_to_inv in H; firstorder congruence.
-Qed.
-
-Ltac commit := repeat (setoid_rewrite refine_Permutation_Reflexivity
-                    || setoid_rewrite refine_Count
-                    || setoid_rewrite refine_MaxN
-                    || setoid_rewrite refine_SumN
-                    || setoid_rewrite refine_MaxZ
-                    || setoid_rewrite refine_SumZ
-                    || setoid_rewrite refine_Max
-                    || setoid_rewrite refine_Sum);
-              try (etransitivity; [ apply refine_count | ]);
-              cleanup; try simplify with monad laws.
-
-(* Next, a trivial step to choose the new database to be just the old one. *)
-
-Ltac choose_db AbsR := unfold AbsR; rewrite refine_pick_val by eauto; [ simplify with monad laws ].
-
-(* Final wrapper tactic for observers *)
-
-Ltac storageOf T :=
-  match eval hnf in T with
-    | (?T1 * ?T2)%type =>
-      let s1 := storageOf T1 in
-      let s2 := storageOf T2 in
-      constr:(s1, s2)
-    | _ =>
-      match eval unfold T in T with
-        | ?s => s
-      end
+Ltac find_equivalent_tuple schemas heading k :=
+  match schemas with
+    | nil => fail
+    | ?sch' :: ?schemas' =>
+      (let H := fresh in
+       assert (schemaHeading (relSchema sch') = heading) as H
+           by reflexivity;
+       clear H;  k (relName sch'))
+        || find_equivalent_tuple schemas' heading k
   end.
 
-Ltac observer' AbsR storages :=
-  startMethod AbsR; concretize; asPerm storages;
-  commit; choose_db AbsR; finish honing.
-
-Ltac observer :=
-  match goal with
-    | [ _ : ?AbsR _ _ |- _ ] =>
-      match type of AbsR with
-        | UnConstrQueryStructure _ -> ?T -> Prop =>
-          let storages := storageOf T in observer' AbsR storages
-    end
-  end.
-
-(* Tactics for implementing constraint checks in mutators *)
-
-Theorem key_symmetry : forall A H (f : _ -> _ -> Comp A) (P : _ -> Prop) sc1 sc2 n,
-  refine (x1 <- Pick (fun b : bool => decides b (forall tup' : @IndexedTuple H,
-                                                   P tup'
-                                                   -> tupleAgree n (indexedElement tup') sc1
-                                                   -> tupleAgree n (indexedElement tup') sc2));
-          x2 <- Pick (fun b : bool => decides b (forall tup' : @IndexedTuple H,
-                                                    P tup'
-                                                    -> tupleAgree (indexedElement tup') n sc1
-                                                    -> tupleAgree (indexedElement tup') n sc2));
-          f x1 x2)
-         (x1 <- Pick (fun b : bool => decides b (forall tup' : @IndexedTuple H,
-                                                   P tup'
-                                                   -> tupleAgree n (indexedElement tup') sc1
-                                                   -> tupleAgree n (indexedElement tup') sc2));
-          f x1 x1).
-Proof.
-  unfold refine; intros.
-  apply computes_to_inv in H0; firstorder.
-  apply computes_to_inv in H0; firstorder.
-  econstructor.
-  eauto.
-  econstructor.
-  econstructor.
-  instantiate (1 := x).
-  eapply decide_eq_iff_iff_morphism; eauto.
-  unfold tupleAgree; intuition auto using sym_eq.
-  assumption.
-Qed.
-
-Ltac pruneDuplicates :=
-  repeat ((setoid_rewrite refine_trivial_if_then_else
-           || setoid_rewrite key_symmetry
-           || setoid_rewrite refine_tupleAgree_refl_True); try simplify with monad laws).
-
-(* Pick a new logical index using [EnsembleBagEquivalence_pick_new_index] *)
-Ltac pickIndex :=
-    match goal with
-        [H : EnsembleBagEquivalence ?storage ?R ?bag
-         |- context[Pick (fun bound => UnConstrFreshIdx ?R bound) ] ] =>
-        let bound := fresh in
-        let ValidBound := fresh in
-        destruct (@EnsembleBagEquivalence_pick_new_index _ storage R bag H)
-          as [bound ValidBound];
-          rewrite refine_pick_val by eauto using ValidBound;
-          simplify with monad laws end.
-
-Ltac revealSchema :=
-  repeat match goal with
-         | [ x : ?T |- _ ] =>
-           match T with
-           | _#_ => fail 1
-           | _ => red in x; match type of x with
-                            | _#_ => idtac
+Ltac find_equivalent_search_term_pair m n build_search_term_dep :=
+match goal with
+    [ H : @DelegateToBag_AbsR ?qs_schema ?indices ?r_o ?r_n
+      |- ExtensionalEq ?f _ ] =>
+    get_ithDefault_pair f m n
+      ltac:(fun filter_dec =>
+        let dom := match type of filter_dec with
+                     | ?A -> ?B -> bool => constr:(A)
+                   end in
+        let heading := match type of filter_dec with
+                         | ?A -> @Tuple ?heading -> bool => constr:(heading)
+                       end in
+        let schemas := eval simpl in (qschemaSchemas qs_schema) in
+            find_equivalent_tuple schemas heading
+              ltac:(fun id => let idx' := constr:({| bindex := id |} : BoundedIndex (map relName (qschemaSchemas qs_schema)))
+                              in let idx := eval simpl in idx' in
+    let idx_search_update_term := eval simpl in (ith_Bounded relName indices idx) in
+    let search_term_type := eval simpl in (BagSearchTermType idx_search_update_term) in
+        let search_term_matcher := eval simpl in (BagMatchSearchTerm idx_search_update_term) in
+        makeEvar (dom -> search_term_type)
+                 ltac: (fun search_term =>
+                          let eqv := fresh in
+                          assert (forall a b, filter_dec a b
+                                                = search_term_matcher (search_term a) b) as eqv;
+                        [ build_search_term_dep qs_schema idx
+                          dom filter_dec search_term
+                        | match goal with
+                            |- ExtensionalEq ?f ?search_term' =>
+                            match type of f with
+                                | ?A -> _ =>
+                                  unify search_term' (fun a : A => search_term_matcher (search_term (ith_default unit_Heading unit_Tuple a m))
+            ((ith_default unit_Heading unit_Tuple a n)))
                             end
-           end
-         end.
+                                                  end;
+                          unfold ExtensionalEq in *; intros;
+                          simpl in *; rewrite eqv; reflexivity
+]))) end.
 
-Ltac foreignToQuery :=
-  revealSchema;
-  match goal with
-    | [ _ : ?SC#_ |- context[Pick
-                               (fun b' =>
-                                  decides
-                                    b'
-                                    (ForeignKey_P ?attr ?attr'
-                                                  ?tupmap ?tup
-                                                  (_!?R)%QueryImpl))]]
-      =>  let T' := constr:(@Tuple (schemaHeading
-                                      (relSchema
-                                         (@nth_Bounded NamedSchema string relName (qschemaSchemas SC) ``R)))) in
-      let temp := fresh in
-      pose (refine_foreign_key_check_into_query (fun t : T' => tup attr = tupmap (t attr'))) as temp; unfold ForeignKey_P;
-      rewrite temp by eauto with typeclass_instances;
-        simplify with monad laws; cbv beta; simpl; clear temp
-  end.
+Ltac find_equivalent_search_term m build_search_term :=
+match goal with
+    [ H : @DelegateToBag_AbsR ?qs_schema ?indices ?r_o ?r_n
+      |- ExtensionalEq ?f _ ] =>
+    get_ithDefault f m
+      ltac:(fun filter_dec =>
+        let heading := match type of filter_dec with
+                         | @Tuple ?heading -> bool => constr:(heading)
+                       end in
+        let schemas := eval simpl in (qschemaSchemas qs_schema) in
+            find_equivalent_tuple schemas heading
+              ltac:(fun id => let idx' := constr:({| bindex := id |} : BoundedIndex (map relName (qschemaSchemas qs_schema)))
+                              in let idx := eval simpl in idx' in
+    let idx_search_update_term := eval simpl in (ith_Bounded relName indices idx) in
+    let search_term_type := eval simpl in (BagSearchTermType idx_search_update_term) in
+        let search_term_matcher := eval simpl in (BagMatchSearchTerm idx_search_update_term) in
+        makeEvar (search_term_type)
+                 ltac: (fun search_term =>
+                          let eqv := fresh in
+                          assert (forall a, filter_dec a
+                                                = search_term_matcher search_term a) as eqv;
+                        [ build_search_term qs_schema idx
+                          filter_dec search_term
+                        | match goal with
+                              |- ExtensionalEq ?f ?search_term' =>
+                              match type of f with
+                                | ?A -> _ =>
+                                  unify search_term' (fun a : A => search_term_matcher search_term (ith_default unit_Heading unit_Tuple a m))
+                              end
+                          end;
+                          unfold ExtensionalEq in *; intros;
+                          simpl in *; rewrite eqv; reflexivity
+]))) end.
 
-Ltac dec_tauto := clear; intuition eauto;
-                  eapply Tuple_Agree_eq_dec;
-                  match goal with
-                    | [ |- ?E = true ] => case_eq E; intuition idtac; [ exfalso ]
-                  end;
-                  match goal with
-                    | [ H : _ |- _ ] => apply Tuple_Agree_eq_dec' in H; solve [ eauto ]
-                  end.
 
-Ltac fundepToQuery :=
-  match goal with
-    | [ |- context[Pick (fun b => decides b (forall tup', _ -> tupleAgree ?n _ _ -> tupleAgree ?n _ _))] ] =>
-      rewrite (refine_functional_dependency_check_into_query n);
-        [ | prove_decidability_for_functional_dependencies | dec_tauto ]
-    | [ |- context[Pick (fun b => decides b (forall tup', _ -> tupleAgree _ ?n _ -> tupleAgree _ ?n _))] ] =>
-      rewrite (refine_functional_dependency_check_into_query n);
-        [ | prove_decidability_for_functional_dependencies | dec_tauto ]
-  end; try simplify with monad laws.
+Corollary refine_Join_Lists_filter_filter_search_term_snd_dep'
+          qs_schema BagIndexKeys
+        (ResultT : Type) :
+    forall (r_n : IndexedQueryStructure qs_schema BagIndexKeys)
+           idx idx'
+           (search_pattern : _ -> _)
+           (resultComp : ilist (@Tuple) [_; _] -> Comp (list ResultT))
+           filter_rest st,
+      refine (cl <- CallBagMethod idx {| bindex := "Find" |} r_n st;
+              l' <- (Join_Lists (Build_single_Tuple_list (snd cl))
+                                (fun _ => l <- CallBagMethod idx' {| bindex := "Enumerate" |} r_n ();
+                                 ret (snd l)));
+              List_Query_In (filter (fun a : ilist (@Tuple) [_ ; _] => BagMatchSearchTerm _ (search_pattern (ilist_tl a)) (ilist_hd a) && filter_rest a) l')
+                            resultComp)
+             (cl <- CallBagMethod idx {| bindex := "Find" |} r_n st;
+              l' <- (Join_Lists (Build_single_Tuple_list (snd cl))
+                                (fun tup => l <- CallBagMethod idx' {| bindex := "Find" |} r_n (search_pattern tup);
+                                             ret (snd l)));
+                      List_Query_In (filter filter_rest l') resultComp).
+  Proof.
+    intros; f_equiv; intro;
+    apply refine_Join_Lists_filter_search_term_snd_dep.
+  Qed.
 
-Ltac checksSucceeded :=
-  match goal with
-    | [ |- context[ret (_, true)] ] =>
-      setoid_rewrite refineEquiv_pick_pair;
-        (* Because our equivalence relation on Bags hides the application of ,
-           benumerate, we can now simply call [refineEquiv_pick_pair]
-           instead of  [refineEquiv_pick_pair_benumerate]  here.  *)
-        simplify with monad laws;
-      repeat (rewrite refine_pick_val by
-                 (refine_bag_update_other_table
-                    || binsert_correct_DB);
-              simplify with monad laws);
-      reflexivity
-  end.
-
-Ltac bdeleteZeta :=
-  simpl;
-  match goal with
-    | [ |- refine (ret ?p) ?B ] =>
-      match goal with
-          [ |- context[@bdelete ?bag ?item ?TSearchTerm ?UpdateTerm
-                           ?bag_proof ?r_n ?search_term] ] =>
-          let b :=
-              (eval pattern (@bdelete bag item TSearchTerm UpdateTerm bag_proof r_n search_term)
-                in p) in
-          match b with
-              | ?g ?x => change p with (let y := x in g y);
-                         cbv beta
-          end
-      end
-  end.
-
-Ltac deleteChecksSucceeded :=
-  useDeleteIndex;
-  match goal with
-    | [ |- context[ret (_, fst (bdelete ?r_n ?search_term)) ] ] =>
-      setoid_rewrite refineEquiv_pick_pair;
-        simplify with monad laws;
-        repeat (rewrite refine_pick_val
-                by (simpl; (refine_bag_update_other_table
-                              || snd_bdelete_correct search_term));
-                simplify with monad laws);
-        bdeleteZeta
-  end.
-
-Ltac checksFailed :=
-  match goal with
-    | [ |- context[ret (_, false)] ] =>
-      rewrite refine_pick_val by eauto; simplify with monad laws; reflexivity
-  end.
-
-Ltac deleteChecksFailed :=
-  match goal with
-    | [ |- context[ret (_, [])] ] =>
-      simplify with monad laws;
-        rewrite refine_pick_val by eauto; simplify with monad laws;
-        simpl; reflexivity
-  end.
-
-Ltac mutator' AbsR storages :=
-  startMethod AbsR; pruneDuplicates; pickIndex;
-  repeat ((foreignToQuery || fundepToQuery);
-          concretize; asPerm storages; commit);
-  Split Constraint Checks; checksSucceeded || checksFailed.
-
-Ltac mutator :=
-  match goal with
-    | [ |- context[UnConstrFreshIdx _ _] ] =>
-      match goal with
-        | [ |- context[nr' <- Pick (fun nr' => ?AbsR _ nr'); ret (nr', _)] ] =>
-          match type of AbsR with
-            | UnConstrQueryStructure _ -> ?T -> Prop =>
-              let storages := storageOf T in mutator' AbsR storages
-          end
-      end
-  end.
-
-(* Now, one tactic to combine all method types. *)
-
-Ltac method :=
-  match goal with
-    | [ |- refine (x <- ret _; Pick _) _ ] => initializer
-    | [ |- refine (x <- _; y <- Pick _; ret _) _ ] => observer
-    | _ => mutator
-  end.
-
-Ltac honeOne :=
-  match goal with
-    | [ |- context[@Build_consDef _ (Build_consSig ?id _) _] ] =>
-      hone constructor id; [ method | ]
-    | [ |- context[@Build_methDef _ (Build_methSig ?id _ _) _] ] =>
-      hone method id; [ method | ]
-  end.
-
-(* Finally, implement a whole ADT. *)
-
-Ltac unfolder E k :=
-  (let E' := eval unfold E in E in k E')
-    || k E.
-
-Ltac hone_representation AbsR' :=
-  eapply SharpenStep;
-  [eapply refineADT_BuildADT_Rep_default with (AbsR := AbsR') |
-   compute [imap absConsDef absMethDef]; simpl ].
-
-Ltac plan AbsR :=
-  match goal with
-    | [ |- Sharpened ?spec ] =>
-      unfolder spec ltac:(fun spec' => change spec with spec')
-  end; start_honing_QueryStructure; hone_representation AbsR;
-  repeat honeOne.
-
-Ltac delete_preserves_primary_keys :=
+  Ltac convert_filter_to_find':=
+    try match goal with
+            |- context[filter (fun a => (_ && _) && true) _] =>
+            setoid_rewrite <- andb_assoc; simpl
+        end;
     match goal with
-        [ |- context [{b |
-            ((forall tup tup',
-                GetUnConstrRelation ?or ?Ridx tup
-                -> GetUnConstrRelation ?or ?Ridx tup' ->
-                FunctionalDependency_P ?attr1 ?attr2 _ _)
-             -> decides b (DeletePreservesSchemaConstraints
-                     (GetUnConstrRelation ?or ?Ridx) ?DeletedTuples
-                     ?P)) }]] =>
-        rewrite (@DeletePrimaryKeysOK _ or Ridx DeletedTuples
-                   attr1 attr2); simplify with monad laws
+      | H : @DelegateToBag_AbsR ?qs_schema ?indices ?r_o ?r_n
+        |- context[l <- CallBagMethod ?idx ``("Enumerate") ?r_n ();
+                    List_Query_In (filter (fun a => MatchIndexSearchTerm ?st (ilist_hd a) && @?filter_rest a)
+                                          (Build_single_Tuple_list (snd l))) ?resultComp] =>
+        let b := fresh in
+        pose proof (@refine_Query_For_In_Find_single _ _ _ r_o r_n H idx st resultComp filter_rest) as b;
+          simpl in b; setoid_rewrite b; clear b
+
+      | H : @DelegateToBag_AbsR ?qs_schema ?indices ?r_o ?r_n
+        |- context[l <- CallBagMethod ?idx ``("Enumerate") ?r_n ();
+                    l' <- Join_Lists (Build_single_Tuple_list (snd l)) ?cl;
+                    List_Query_In (filter (fun a => MatchIndexSearchTerm ?st (ilist_hd (ilist_tl a)) && @?filter_rest a)
+                                          l') ?resultComp] =>
+        let b := fresh in
+        pose proof (fun foo => @refine_Join_Lists_filter_search_term_fst _ _ _ r_n idx _ cl st resultComp foo filter_rest) as b;
+          simpl in b; setoid_rewrite b;
+          [ clear b
+          | match goal with
+              | |- context [CallBagMethod ?idx' ``("Enumerate") _ _] =>
+                intros; eapply (realizeable_Enumerate (r_o := r_o) (r_n := r_n) idx' H)
+              | |- context [CallBagMethod ?idx' ``("Find") _ _] =>
+                intros; eapply (realizeable_Find (r_o := r_o) (r_n := r_n) idx' H)
+            end]
+      | H : @DelegateToBag_AbsR ?qs_schema ?indices ?r_o ?r_n
+        |- context[l <- CallBagMethod ?idx ``("Find") ?r_n ?st;
+                    l' <- Join_Lists (Build_single_Tuple_list (snd l))
+                       (fun _ : ilist (@Tuple) [?heading] =>
+                          l <- CallBagMethod ?idx' ``("Enumerate") ?r_n ();
+                        ret (snd l));
+                    List_Query_In (filter (fun a => MatchIndexSearchTerm (Dep_SearchTerm_Wrapper ?st' (ilist_hd (ilist_tl a)))
+                                                                         (ilist_hd a) && @?filter_rest a) l') ?resultComp] =>
+        let b := fresh in
+        pose proof (@refine_Join_Lists_filter_filter_search_term_snd_dep' _ _ _ r_n idx idx'
+                                                                          (fun a => Dep_SearchTerm_Wrapper st' (ilist_hd a))
+                                                                          resultComp filter_rest st) as b;
+          unfold Dep_SearchTerm_Wrapper in b; simpl in b; setoid_rewrite b; clear b
+      (* The final case replaces the last filter and the Return statement. *)
+      | _ => setoid_rewrite filter_true; setoid_rewrite refine_List_Query_In_Return
     end.
 
-Ltac delete_foreign_key_check_to_Query storage :=
+  Ltac convert_filter_to_find :=
+    simpl; repeat convert_filter_to_find'.
+
+  (* This also implements Fors *)
+  Ltac Implement_Aggregates :=
+    repeat
+      match goal with
+        | |- context[For _] => setoid_rewrite refine_For_List
+        | |- context[Count _] => setoid_rewrite refine_Count
+      end.
+
+  (* Commits the database at the end of a method call. *)
+  Ltac commit :=
     match goal with
-        [ |- context [
-                 {b'|
-                           ?P ->
-                           decides b'
-                             (DeletePreservesCrossConstraints
-                                (GetUnConstrRelation ?qs ?Ridx)
-                                (GetUnConstrRelation ?qs ?Ridx')
-                                ?DeletedTuples
-                                (ForeignKey_P ?attr1 ?attr2 ?tupmap))} ]
-        ] => rewrite (@DeleteForeignKeysCheck _ qs Ridx Ridx'
-                                                 DeletedTuples)
-    end;
-      [simplify with monad laws;
-        concretize;
-        asPerm storage;
-        commit
-      | auto with typeclass_instances
-      | unfold tupleAgree; clear; simpl;
-        let H' := fresh in intros; rewrite <- H'; eauto
-      | auto with typeclass_instances
-      | unfold Iterate_Ensemble_BoundedIndex_filter; simpl; intuition
-      | simpl; auto
-      ]. *)
+      | [H : @DelegateToBag_AbsR ?qs_schema ?indices ?r_o ?r_n
+         |- context[{r_n' : IndexedQueryStructure ?qs_schema ?indices | DelegateToBag_AbsR ?r_o r_n'}] ]
+        => setoid_rewrite (refine_pick_val (@DelegateToBag_AbsR qs_schema indices r_o) H);
+          simplify with monad laws
+    end.
